organize enum.v

model/Enum.v
@@ -90,190 +90,209 @@ Inductive Enum : Set :=
 
 Hint Constructors Enum.
 
-Inductive Pairing : nat -> nat -> nat -> Prop :=
-| P_XBig :
-  forall x y,
-    y <= x ->
-    Pairing (x*x + x + y) x y
-| P_XSmall :
-  forall x y,
-    x < y ->
-    Pairing (x + y*y) x y.
-Hint Constructors Pairing.
+Section Pairing.
+  Inductive Pairing : nat -> nat -> nat -> Prop :=
+  | P_XBig :
+    forall x y,
+      y <= x ->
+      Pairing (x*x + x + y) x y
+  | P_XSmall :
+    forall x y,
+      x < y ->
+      Pairing (x + y*y) x y.
+  Hint Constructors Pairing.
 
-Theorem Pairing_lt :
-  forall m n p,
-    Pairing p m n -> (m = 0 /\ n <= 1) \/ (m <= 1 /\ n = 0) \/ (p > m /\ p > n).
-Proof.
-  intros m n p P.
-  inversion P; subst; nliamega.
-Qed.
+  Theorem Pairing_lt :
+    forall m n p,
+      Pairing p m n -> (m = 0 /\ n <= 1) \/ (m <= 1 /\ n = 0) \/ (p > m /\ p > n).
+  Proof.
+    intros m n p P.
+    inversion P; subst; nliamega.
+  Qed.
 
-Theorem Pairing_from_fun :
-  forall l r n1 n2,
-    Pairing n1 l r ->
-    Pairing n2 l r ->
-    n1 = n2.
-Proof.
-  intros l r n1 n2 P1 P2.
-  inversion P1; inversion P2; subst; nliamega.
-Qed.
+  Theorem Pairing_from_fun :
+    forall l r n1 n2,
+      Pairing n1 l r ->
+      Pairing n2 l r ->
+      n1 = n2.
+  Proof.
+    intros l r n1 n2 P1 P2.
+    inversion P1; inversion P2; subst; nliamega.
+  Qed.
 
-Lemma Pairing_to_incompat:
-  forall l1 l2 r1 r2,
-    r1 <= l1 ->
-    l2 < r2 ->
-    l2 + r2 * r2 = l1 * l1 + l1 + r1 ->
-    False.
-Proof.
-  intros; destruct (eq_nat_dec r2 l1); subst; nliamega.
-Qed.
+  Lemma Pairing_to_incompat:
+    forall l1 l2 r1 r2,
+      r1 <= l1 ->
+      l2 < r2 ->
+      l2 + r2 * r2 = l1 * l1 + l1 + r1 ->
+      False.
+  Proof.
+    intros; destruct (eq_nat_dec r2 l1); subst; nliamega.
+  Qed.
 
-Theorem Pairing_to_fun :
-  forall n l1 l2 r1 r2,
-    Pairing n l1 r1 ->
-    Pairing n l2 r2 ->
-    (l1 = l2) /\ (r1 = r2).
-Proof.
-  intros n l1 l2 r1 r2 P1 P2.
-  inversion P1; inversion P2; clear P1; clear P2; subst.
+  Theorem Pairing_to_fun :
+    forall n l1 l2 r1 r2,
+      Pairing n l1 r1 ->
+      Pairing n l2 r2 ->
+      (l1 = l2) /\ (r1 = r2).
+  Proof.
+    intros n l1 l2 r1 r2 P1 P2.
+    inversion P1; inversion P2; clear P1; clear P2; subst.
 
-  replace l1 with l2 in * by nliamega.
-  replace r1 with r2 in * by nliamega.
-  auto.
+    replace l1 with l2 in * by nliamega.
+    replace r1 with r2 in * by nliamega.
+    auto.
 
-  cut False. contradiction.
-  eapply (Pairing_to_incompat _ _ _ _ H H3 H4).
+    cut False. contradiction.
+    eapply (Pairing_to_incompat _ _ _ _ H H3 H4).
 
-  cut False. contradiction.
-  symmetry in H4.
-  eapply (Pairing_to_incompat _ _ _ _ H3 H H4).
+    cut False. contradiction.
+    symmetry in H4.
+    eapply (Pairing_to_incompat _ _ _ _ H3 H H4).
 
-  replace r1 with r2 in * by nliamega.
-  replace l1 with l2 in * by nliamega.
-  auto.
-Qed.
+    replace r1 with r2 in * by nliamega.
+    replace l1 with l2 in * by nliamega.
+    auto.
+  Qed.
 
-Theorem Pairing_to_l_fun :
-  forall n l1 l2 r1 r2,
-    Pairing n l1 r1 ->
-    Pairing n l2 r2 ->
-    l1 = l2.
-Proof.
-  intros n l1 l2 r1 r2 P1 P2.
-  edestruct (Pairing_to_fun _ _ _ _ _ P1 P2). auto.
-Qed.
-Theorem Pairing_to_r_fun :
-  forall n l1 l2 r1 r2,
-    Pairing n l1 r1 ->
-    Pairing n l2 r2 ->
-    r1 = r2.
-Proof.
-  intros n l1 l2 r1 r2 P1 P2.
-  edestruct (Pairing_to_fun _ _ _ _ _ P1 P2). auto.
-Qed.
+  Theorem Pairing_to_l_fun :
+    forall n l1 l2 r1 r2,
+      Pairing n l1 r1 ->
+      Pairing n l2 r2 ->
+      l1 = l2.
+  Proof.
+    intros n l1 l2 r1 r2 P1 P2.
+    edestruct (Pairing_to_fun _ _ _ _ _ P1 P2). auto.
+  Qed.
+  Theorem Pairing_to_r_fun :
+    forall n l1 l2 r1 r2,
+      Pairing n l1 r1 ->
+      Pairing n l2 r2 ->
+      r1 = r2.
+  Proof.
+    intros n l1 l2 r1 r2 P1 P2.
+    edestruct (Pairing_to_fun _ _ _ _ _ P1 P2). auto.
+  Qed.
 
-Theorem Pairing_to_dec:
-  forall x y,
-    { n | Pairing n x y }.
-Proof.
-  intros x y.
-  destruct (le_lt_dec y x) as [BIG | SMALL]; eauto.
-Defined.
+  Theorem Pairing_to_dec:
+    forall x y,
+      { n | Pairing n x y }.
+  Proof.
+    intros x y.
+    destruct (le_lt_dec y x) as [BIG | SMALL]; eauto.
+  Defined.
 
-Definition Pairing_to x y : nat := proj1_sig (Pairing_to_dec x y).
-Corollary Pairing_to_sound :
-  forall l r,
-    Pairing (Pairing_to l r) l r.
-Proof.
-  intros l r. unfold Pairing_to.
-  remember (Pairing_to_dec l r) as vn.
-  destruct vn as [n P]. simpl. auto.
-Qed.
-Hint Resolve Pairing_to_sound.
+  Definition Pairing_to x y : nat := proj1_sig (Pairing_to_dec x y).
+  Corollary Pairing_to_sound :
+    forall l r,
+      Pairing (Pairing_to l r) l r.
+  Proof.
+    intros l r. unfold Pairing_to.
+    remember (Pairing_to_dec l r) as vn.
+    destruct vn as [n P]. simpl. auto.
+  Qed.
+  Hint Resolve Pairing_to_sound.
 
-Lemma sqrt_lemma z : (z - (sqrt z * sqrt z)) - sqrt z <= sqrt z.
-Proof.
-  induction z; try nliamega.
-  SearchAbout "le_".
-  destruct (Nat.sqrt_succ_or z).
-  nliamega.
-  remember (Nat.sqrt_succ_le z).
-  clear Heql.
-  rewrite H at 1 2 3.
-  assert (z - sqrt z * sqrt z - sqrt z < sqrt z). admit.
-  clear IHz l.
-  nliamega.
-Qed.
+  Section Sqrt.
+    Lemma sqrt_lemma z : (z - (sqrt z * sqrt z)) - sqrt z <= sqrt z.
+    Proof.
+      induction z; try nliamega.
+      SearchAbout "le_".
+      destruct (Nat.sqrt_succ_or z).
+      nliamega.
+      remember (Nat.sqrt_succ_le z).
+      clear Heql.
+      rewrite H at 1 2 3.
+      assert (z - sqrt z * sqrt z - sqrt z < sqrt z). admit.
+      clear IHz l.
+      nliamega.
+    Qed.
+
+    Lemma sqrt_lemma' z :
+      (z - (sqrt z) * (sqrt z) < (sqrt z))
+      -> z = z - (sqrt z * sqrt z) + (sqrt z * sqrt z).
+    Proof.
+      remember (sqrt_spec z); nliamega.
+    Qed.
+
+    Lemma sqrt_lemma'' k n :
+      (n * n <= k < S n * S n) -> k - sqrt k * sqrt k - sqrt k < S n.
+    Proof.
+      intros H; rewrite (Nat.sqrt_unique k n); lia.
+    Qed.
+
+    Lemma sqrt_slower_than_id' n :
+      (S (sqrt (S (4 + n)))) < 4 + n.
+    Proof.
+      induction n.
+      compute; reflexivity.
+      assert (sqrt (S (4 + S n)) <= (S (S (S n)))); [| nliamega].
+      eapply le_trans; [apply Nat.sqrt_succ_le|].
+      replace (4 + S n) with (S (4 + n)) by nliamega.
+      nliamega.
+    Qed.
+
+    Lemma sqrt_slower_than_id n :
+      4 <= n ->
+      (S (sqrt (S n))) < n.
+    Proof.
+      intros H.
+      replace n with (4 + (n - 4)) by nliamega.
+      apply sqrt_slower_than_id'.
+    Qed.
+
+    Lemma sqrt_spec_2 n :
+      16 <= n ->
+      exists m p,
+        m * m <= n < (p * p) * (p * p) /\ p * p < m * m.
+    Proof.
+      intros H.
+      exists (S (S (sqrt (S (sqrt n))))).
+      exists (S (sqrt (S (sqrt n)))).
+      split; [| nliamega].
+      split; [| destruct (sqrt_spec n); destruct (sqrt_spec (S (sqrt n))); nliamega ].
+      destruct (sqrt_spec n).
+      apply le_trans with (m := sqrt n * sqrt n); auto.
+      assert (S (S (sqrt (S (sqrt n)))) <= sqrt n) as Hperf; [|(apply mult_le_compat; apply Hperf)].
+      assert (4 <= sqrt n).
+      replace 4 with (sqrt 16) .
+      apply Nat.sqrt_le_mono; auto.
+      compute; trivial.
+      apply sqrt_slower_than_id; auto.
+    Qed.
+
+    Lemma nat_le_iff : forall m p, (forall q : nat, q <= m -> q <= p) <-> m <= p.
+    Proof.
+      split.
+      intros H. apply (H m); auto.
+      intros H q; nliamega.
+    Qed.
+
+    Lemma nat_lt_iff : forall m p, (forall q : nat, q < m -> q < p) <-> m <= p.
+    Proof.
+      destruct m.
+      intros p; split; [nliamega| intros _ q contra; inversion contra].
+      destruct p.
+      split.
+      intros contra; assert (m < 0) by (apply contra; auto); nliamega.
+      intros contra; inversion contra.
+      split.
+      intros H.
+      assert (m <= p); [| nliamega].
+      apply nat_le_iff.
+      intros q Hqm.
+      assert (q < S p); [| nliamega].
+      apply H; nliamega.
+      intros; nliamega.
+    Qed.
 
 
-Lemma sqrt_lemma' z :
-  ((z - (sqrt z * sqrt z)) - sqrt z <= sqrt z /\ sqrt (S z) = S (sqrt z))
-  \/ ((z - (sqrt z * sqrt z)) - sqrt z < sqrt z /\ sqrt (S z) = sqrt z)
-.
-Proof.
-  induction z; [compute; intuition|].
-  destruct IHz as [[? ?] | [? ?]].
-  right; split.
-  nliamega.
-  admit.
+  End Sqrt.
 
-  destruct (eq_nat_dec (sqrt (S (S z))) (sqrt (S z))).
-  right; split.
-  
-  (* right; split. *)
-  (* remember (Nat.sqrt_succ_le z). *)
-  (* clear Heql. *)
-  (* rewrite H0 at 1 2 3. *)
-(*  H : sqrt (S z) = sqrt z
-  H0 : z - sqrt z * sqrt z - sqrt z < sqrt z
-  ============================
-   S z - sqrt z * sqrt z - sqrt z <= sqrt (S z)
- *)  
-(*   z : nat
-  IHz : z - sqrt z * sqrt z - sqrt z <= sqrt z
-  H : sqrt (S z) = sqrt z
-  l : sqrt (S z) <= S (sqrt z)
-  H0 : z - sqrt z * sqrt z - sqrt z < sqrt z
-  ============================
-   S z - sqrt z * sqrt z - sqrt z <= sqrt (S z)
-*)
-  (* left; split. *)
-  (* nliamega. *)
-  
-  (* left. *)
-  (* split. *)
-  (* nliamega. *)
-  (* rewrite H0. *)
-  (* admit. (* sqrt (n+1) = (sqrt n)+1 -> sqrt (n+2) = (sqrt) *) *)
-  (* right. *)
-  (* split. *)
-
-  (* admit. *)
-  (* nliamega. *)
-  (* remember (Nat.sqrt_succ_le z). *)
-  (* remember (Nat.sqrt_succ_le (S z)). *)
-  (* nliamega. *)
-  (* nliamega. *)
-Abort.
-
-Lemma sqrt_lemma' z :
-  (z - (sqrt z) * (sqrt z) < (sqrt z))
-  -> z = z - (sqrt z * sqrt z) + (sqrt z * sqrt z).
-Proof.
-  remember (sqrt_spec z); nliamega.
-Qed.
-
-Lemma sqrt_lemma'' k n :
-  (n * n <= k < S n * S n) -> k - sqrt k * sqrt k - sqrt k < S n.
-Proof.
-  intros H; rewrite (Nat.sqrt_unique k n); lia.
-Qed.
-
-Theorem Pairing_from_dec:
-  forall n,
-    { xy | Pairing n (fst xy) (snd xy) }.
-Proof.
+  Theorem Pairing_from_dec:
+    forall n,
+      { xy | Pairing n (fst xy) (snd xy) }.
+  Proof.
   (* (z - rootz^2, rootz)          if z - rootz^2 <  rootz
      (rootz, (z - rootz^2) -rootz) if z - rootz^2 >= rootz
    *)
@@ -298,1690 +317,1608 @@ Proof.
   subst.
   rewrite sqrt_lemma' at 1; [| auto].
   simpl; constructor 2; auto.
-Defined.
+  Defined.
 
-(* Eval compute in (Pairing_from_dec 0). *)
-(* Eval compute in (Pairing_from_dec 1). *)
-(* Eval compute in (Pairing_from_dec 2). *)
-(* Eval compute in (Pairing_from_dec 3). *)
-(* Eval compute in (Pairing_from_dec 4). *)
-(* Eval compute in (Pairing_from_dec 5). *)
-(* Eval compute in (Pairing_from_dec 6). *)
-(* Eval compute in (Pairing_from_dec 7). *)
-(* Eval compute in (Pairing_from_dec 8). *)
-(* Eval compute in (Pairing_from_dec 9). *)
-(* Eval compute in (Pairing_from_dec 10). *)
-(* Eval compute in (Pairing_from_dec 11). *)
-
-Definition Pairing_from n : (nat * nat) := proj1_sig (Pairing_from_dec n).
-Corollary Pairing_from_sound :
-  forall n l r,
-    (l, r) = Pairing_from n ->
-    Pairing n l r.
-Proof.
-  intros n l r. unfold Pairing_from.
-  remember (Pairing_from_dec n) as vlr.
-  destruct vlr as [[l' r'] P]. simpl in *.
-  intros EQ. congruence.
-Qed.
+  Definition Pairing_from n : (nat * nat) := proj1_sig (Pairing_from_dec n).
+  Corollary Pairing_from_sound :
+    forall n l r,
+      (l, r) = Pairing_from n ->
+      Pairing n l r.
+  Proof.
+    intros n l r. unfold Pairing_from.
+    remember (Pairing_from_dec n) as vlr.
+    destruct vlr as [[l' r'] P]. simpl in *.
+    intros EQ. congruence.
+  Qed.
+End Pairing.
+(* TODO: find out how to make hints go out of their section *)
+Hint Constructors Pairing.
+Hint Resolve Pairing_to_sound.
 Hint Resolve Pairing_from_sound.
 
 Notation set' := (set nat).
-Inductive Trace :=
-| Tracing : set' -> set' -> set' -> set' -> Trace.
+Notation empty_set' := (@empty_set nat).
+Notation set_union' := (@set_union nat eq_nat_dec).
+Notation set_add' := (@set_add nat eq_nat_dec).
+Section Sets.
+  Fixpoint subset (s1 s2 : set nat) :=
+    match s1 with
+      | nil => True
+      | x :: more =>
+        set_In x s2 /\ subset more s2
+    end.
+  Hint Unfold subset.
 
-Definition trace_proj tg t :=
-  match t with
-    | Tracing t0 t1 t2 t3 =>
-      match tg with
-        | zero  => t0
-        | one   => t1
-        | two   => t2
-        | three => t3
-      end
-  end.
+  Theorem subset_nil : forall s, subset nil s.
+  Proof.
+    auto.
+  Qed.
 
-Definition empty_set' := @empty_set nat.
-Definition set_union' := @set_union nat eq_nat_dec.
-Definition set_add' := @set_add nat eq_nat_dec.
+  Theorem subset_nil_nil : forall s, subset s nil -> s = nil.
+  Proof.
+    induction s.
+    auto.
+    intros contra.
+    unfold subset in contra.
+    destruct contra.
+    inversion H.
+  Qed.
 
-Definition trace_zero : Trace := Tracing empty_set' empty_set' empty_set' empty_set'.
-Definition trace_plus (t1 t2 : Trace) : Trace :=
-  match (t1, t2) with
-    | (Tracing l1 l2 l3 l4, Tracing r1 r2 r3 r4) =>
-      Tracing (set_union' l1 r1)
-              (set_union' l2 r2)
-              (set_union' l3 r3)
-              (set_union' l4 r4)
-  end.
+  Definition set_eq s1 s2 := subset s1 s2 /\ subset s2 s1.
+  Hint Unfold set_eq.
 
-Definition trace_one n t : Trace :=
-  match t with
-    | zero  => Tracing (set_add' n empty_set') empty_set' empty_set' empty_set'
-    | one   => Tracing empty_set' (set_add' n empty_set') empty_set' empty_set'
-    | two   => Tracing empty_set' empty_set' (set_add' n empty_set') empty_set'
-    | three => Tracing empty_set' empty_set' empty_set' (set_add' n empty_set')
-  end.
+  Lemma subset_consr s1 s2 n : subset s1 s2 -> subset s1 (cons n s2).
+  Proof.
+    generalize dependent s2.
+    generalize dependent n.
+    induction s1.
+    constructor.
 
-Inductive Enumerates : Enum -> nat -> Value -> Trace -> Prop :=
-| ES_Nat :
-  forall n,
-    Enumerates E_Nat n (V_Nat n) trace_zero
-| ES_Pair :
-  forall l r n ln rn lx rx lt rt,
-    Pairing n ln rn ->
-    Enumerates l ln lx lt ->
-    Enumerates r rn rx rt ->
-    Enumerates (E_Pair l r) n (V_Pair lx rx) (trace_plus lt rt)
-| ES_Map :
-  forall bi inner inner_x n x t,
-    Bijects bi x inner_x ->
-    Enumerates inner n inner_x t ->
-    Enumerates (E_Map bi inner) n x t
-| ES_Dep:
-  forall l f n ln rn lx rx lt rt,
-    Pairing n ln rn ->
-    Enumerates l ln lx lt ->
-    Enumerates (f lx) rn rx rt ->
-    Enumerates (E_Dep l f) n (V_Pair lx rx) (trace_plus lt rt)
-| ES_Sum_Left:
-  forall l r n ln lx t,
-    n = 2 * ln ->
-    Enumerates l ln lx t ->
-    Enumerates (E_Sum l r) n (V_Sum_Left lx) t
-| ES_Sum_Right:
-  forall l r n rn rx t,
-    n = 2 * rn + 1 ->
-    Enumerates r rn rx t ->
-    Enumerates (E_Sum l r) n (V_Sum_Right rx) t
- (* E_Trace hides traces below it. This makes traces super easily spoofable, but makes it easier to reason about when they're not spoofed *)
-| ES_Trace :
-    forall n tg e v _t,
-      Enumerates e n v _t ->
-      Enumerates (E_Trace tg e) n v (trace_one n tg)
-.
-Hint Constructors Enumerates.
+    intros n s2 H.
+    unfold subset.
+    unfold subset in H.
+    destruct H.
+    fold subset in *.
 
-(* Couldn't prove this with traces assumed to be equal. *)
-Theorem Enumerates_to_fun :
-  forall e x n1 n2 t1 t2,
-    Enumerates e n1 x t1 ->
-    Enumerates e n2 x t2 ->
-    n1 = n2.
-Proof.
-  induction e; intros x n1 n2 t1 t2 E1 E2; inversion E1; inversion E2; subst; try congruence.
+    split.
+    constructor 2; auto.
+    apply IHs1; auto.
+  Defined.
 
-  (* E_Pair *)
-  - replace lx0 with lx in *; try congruence.
-    replace rx0 with rx in *; try congruence.
-    erewrite (IHe1 _ _ _ _ _ H2 H10) in *.
-    erewrite (IHe2 _ _ _ _ _ H6 H14) in *.
-    erewrite (Pairing_from_fun _ _ _ _ H1 H9) in *.
+  Definition subset_dec s1 s2 : { subset s1 s2 } + { ~ (subset s1 s2) }.
+  Proof.
+    generalize dependent s2.
+    induction s1.
+    left; auto.
+
+    intros s2.
+    destruct (In_dec eq_nat_dec a s2).
+
+    destruct (IHs1 s2).
+    left; constructor; auto.
+
+    right.
+    unfold subset; fold subset.
+    intros H; destruct H; contradiction.
+
+    right.
+    intros H; destruct H; contradiction.
+  Defined.
+
+  Definition subset_nn s1 s2 : ~~(subset s1 s2) -> subset s1 s2.
+  Proof.
+    destruct (subset_dec s1 s2); tauto.
+  Qed.
+
+  Definition set_eq_dec s1 s2 : { set_eq s1 s2 } + { ~ (set_eq s1 s2) }.
+  Proof.
+    destruct (subset_dec s1 s2).
+    destruct (subset_dec s2 s1).
+    left; auto.
+    right; intros contra; destruct contra; apply n; auto.
+    right; intros contra; destruct contra; apply n; auto.
+  Qed.
+
+  Theorem subset_refl s : subset s s.
+  Proof.
+    induction s; unfold subset; auto.
+    fold subset.
+    split.
+    constructor 1; auto.
+    apply subset_consr; auto.
+  Qed.
+
+  Theorem set_eq_refl s : set_eq s s.
+  Proof.
+    split; apply subset_refl.
+  Qed.
+
+  Theorem subset_In : forall x s s', set_In x s -> subset s s' -> set_In x s'.
+  Proof.
+    intros x s.
+    generalize dependent x.
+    induction s as [| x s].
+    intros y s contra.
+    inversion contra.
+
+    intros y s' Hyinxs Hsub.
+    destruct Hsub as [Hxins' Hsub].
+    destruct Hyinxs; subst; auto.
+  Qed.
+
+  Theorem subset_In_def s s' : (forall x, set_In x s -> set_In x s') -> subset s s'.
+  Proof.
+    generalize dependent s'.
+    induction s.
+    intros; apply subset_nil.
+    split.
+    apply H; auto.
+    constructor; auto.
+    apply IHs.
+    intros x Hins.
+    apply H.
+    constructor 2; auto.
+  Qed.
+
+  Theorem In_subset_def s s' : subset s s' -> (forall x, set_In x s -> set_In x s').
+  Proof.
+    generalize dependent s'.
+    induction s.
+    intros s' _ x contra.
+    inversion contra.
+
+    intros s' Hsub x Hin.
+    destruct Hin.
+    destruct Hsub; subst.
     auto.
 
-  (* E_Map *)
-  - erewrite (Bijects_fun_right _ _ _ _ _ _ H1 H8) in *.
-    erewrite (IHe _ _ _ _ _ H5 H12) in *.
+    apply IHs.
+    destruct Hsub; subst; auto.
     auto.
+  Qed.
 
-  (* E_Dep *)
-  - inversion H13.
+  Hint Resolve subset_In_def In_subset_def.
+  Theorem subset_In_equiv s s' : subset s s' <-> (forall x, set_In x s -> set_In x s').
+  Proof.
+    split; eauto.
+  Qed.
+
+  Lemma set_subset_weaken : forall s1 s2, set_eq s1 s2 -> subset s1 s2.
+  Proof.
+    unfold set_eq.
+    tauto.
+  Qed.
+
+  Theorem not_subset_In_def s s' x : set_In x s -> ~(set_In x s') -> ~ subset s s'.
+  Proof.
+    intros; eauto.
+  Qed.
+
+  Lemma subset_trans : forall s1 s2 s3, subset s1 s2 -> subset s2 s3 -> subset s1 s3.
+  Proof.
+    intros s1.
+    induction s1 as [| x s1].
+    intros; apply subset_nil.
+    induction s2 as [| y s2].
+    intros s3 contra.
+    inversion contra.
+    inversion H.
+
+    intros s3 Hxy12 Hy23.
+    unfold subset; fold subset.
+    destruct Hxy12 as [Hxy2 H1y2].
+    split.
+
+    eapply subset_In.
+    apply Hxy2.
+    auto.
+    apply IHs1 with (s2 := (y :: s2)); auto.
+  Qed.
+
+
+  Lemma set_eq_trans : forall s1 s2 s3, set_eq s1 s2 -> set_eq s2 s3 -> set_eq s1 s3.
+  Proof.
+    unfold set_eq.
+    intros s1 s2 s3 H1 H2; destruct H1; destruct H2.
+    split; eapply subset_trans; eauto.
+  Qed.
+
+  Lemma set_eq_symm : forall s1 s2, set_eq s1 s2 -> set_eq s2 s1.
+  Proof.
+    intros s1 s2 H; inversion H; split; auto.
+  Qed.
+
+  (* Theorem set_union_or : forall s1 s2, subset s1 (set_union' s1 s2). *)
+
+  Lemma set_add_subset : forall x s1 s2, set_In x s2 -> subset s1 s2 -> subset (set_add' x s1) s2.
+  Proof.
+
+    intros y s1.
+    induction s1 as [| x s1].
+    simpl; auto.
+    intros s2 Hy2 Hsub.
+    unfold set_add.
+    destruct (eq_nat_dec y x); subst; auto.
+    fold set_add.
+    unfold subset.
+    split; auto.
+    destruct Hsub; auto.
+    fold subset.
+    apply IHs1; auto.
+    destruct Hsub; auto.
+  Qed.
+
+  Lemma subset_cons_swap : forall x y s1 s2, subset s1 s2 -> subset (x :: y :: s1) (y :: x :: s2).
+  Proof.
+    intros x y s1 s2.
+    destruct (eq_nat_dec x y).
+    simpl; subst.
+    split.
+    tauto.
+    split.
+    tauto.
+    apply subset_consr.
+    apply subset_consr.
+    assumption.
+
+    simpl.
+    split.
+    tauto.
+    split.
+    tauto.
+    apply subset_consr. apply subset_consr.
+    assumption.
+  Qed.
+
+  Lemma set_eq_cons_swap : forall x y s1 s2, set_eq s1 s2 -> set_eq (x :: y :: s1) (y :: x :: s2).
+  Proof.
+    split; destruct H; apply subset_cons_swap; auto.
+  Qed.
+
+  Lemma set_cons_cons_subset : forall x s1 s2, subset s1 s2 -> subset (x :: s1) (x :: s2).
+  Proof.
+    intros x s1 s2 Hsub.
+    unfold subset. fold subset.
+    split.
+    constructor; auto.
+    apply subset_consr; auto.
+  Qed.
+
+  Lemma set_eq_cons_cons x s1 s2 : set_eq s1 s2 -> set_eq (x :: s1) (x :: s2).
+  Proof.
+    intros H.
+    destruct H.
+    split; apply set_cons_cons_subset; auto.
+  Qed.
+
+  Lemma set_add_cons_eq : forall x s, set_eq (x :: s) (set_add' x s).
+  Proof.
+    split.
+    generalize dependent x.
+    induction s as [| y s].
+    compute; tauto.
+    intros x.
+    simpl.
+    destruct (eq_nat_dec x y); subst.
+    split.
+    constructor; auto.
+    split.
+    constructor; auto.
+    apply subset_consr.
+    apply subset_refl.
+
+    split.
+    destruct (IHs x).
+    apply in_cons. apply H.
+    split.
+    constructor; auto.
+    apply subset_trans with (s2:= (x :: s)).
+    apply subset_consr; auto.
+
+    apply subset_trans with (s2 := (set_add' x s)).
+    apply IHs.
+    apply subset_consr.
+    apply subset_refl.
+
+    generalize dependent x.
+    induction s as [| y s].
+    compute; tauto.
+    intros x.
+    simpl.
+    destruct (eq_nat_dec x y).
+    apply subset_consr.
+    apply subset_refl.
+    apply subset_trans with (y :: x :: s).
+    apply set_cons_cons_subset.
+    apply IHs.
+    apply subset_cons_swap.
+    apply subset_refl.
+  Qed.
+
+  Lemma set_add_cons_subset : forall x s1 s2, subset s1 s2 -> subset (x :: s1) (set_add' x s2).
+  Proof.
+    intros x s1 s2 Hsub.
+    apply subset_trans with (s2 := (x :: s2)).
+    apply set_cons_cons_subset; auto.
+    apply set_subset_weaken.
+    apply set_add_cons_eq.
+  Qed.
+
+  Lemma set_union_unitl : forall s, set_eq (set_union' empty_set' s) s.
+  Proof.
+    split.
+    induction s.
+    apply subset_refl.
+
+    unfold set_union in *.
+    replace (((fix set_union (x y : set nat) {struct y} :
+                 set nat :=
+                 match y with
+                   | nil => x
+                   | a1 :: y1 => set_add eq_nat_dec a1 (set_union x y1)
+                 end) empty_set' s
+            )) with (set_union' empty_set' s) in * by auto.
+    fold set_add'.
+    apply set_add_subset; auto.
+    constructor; auto.
+    apply subset_consr; auto.
+
+    induction s; auto.
+    unfold set_union.
+    fold set_union.
+    apply set_add_cons_subset; auto.
+  Qed.
+
+  Lemma set_union_unitr : forall s, set_eq (set_union' s empty_set') s.
+  Proof.
+    apply set_eq_refl.
+  Qed.
+
+  Lemma elem_union :
+    forall s x,
+      set_In x s -> forall s', set_In x (set_union' s' s).
+  Proof.
+    induction s.
+    intros H contra.
+    inversion contra.
+
+    intros x Hin s'.
+    simpl.
+    assert (set_In x (a :: (set_union' s' s))).
+    destruct Hin.
+    constructor; auto.
+    eapply In_subset_def.
+    apply subset_consr.
+    apply subset_refl.
+    apply IHs; auto.
+    eapply In_subset_def.
+    apply set_add_cons_subset.
+    apply subset_refl.
+    auto.
+  Qed.
+
+  Lemma subset_union_cons : forall x s1 s2, subset (set_union' (x::s1) s2) (x :: (set_union' s1 s2)).
+    induction s2.
+    simpl; split.
+    tauto.
+    apply subset_consr; apply subset_refl.
+    simpl.
+    eapply subset_trans.
+    apply set_add_cons_eq.
+    apply subset_trans with (s2 := (x :: a :: (set_union' s1 s2))).
+    eapply subset_trans.
+    apply set_cons_cons_subset.
+    apply IHs2.
+    apply subset_cons_swap.
+    apply subset_refl.
+    apply set_cons_cons_subset.
+    apply set_add_cons_eq.
+  Qed.
+
+  Theorem subset_union_comm : forall s1 s2, subset (set_union' s1 s2) (set_union' s2 s1).
+  Proof.
+    induction s1.
+    intros.
+    apply subset_trans with (s2 := s2).
+    apply set_union_unitl.
+    apply set_union_unitr.
+
+    intros s2.
+    simpl.
+    eapply subset_trans.
+    apply subset_union_cons.
+    apply set_add_cons_subset.
+    apply IHs1.
+  Qed.
+
+  Theorem set_eq_union_comm : forall s1 s2, set_eq (set_union' s1 s2) (set_union' s2 s1).
+  Proof.
+    intros s1 s2.
+    split; apply subset_union_comm.
+  Qed.
+
+  Lemma subset_union_transr :
+    forall s sl sr,
+      subset s sr ->
+      subset s (set_union' sl sr).
+  Proof.
+    intros.
+    apply subset_In_def.
+    intros x Hin.
+    apply elem_union.
+    eapply In_subset_def.
+    apply H.
+    auto.
+  Qed.
+
+  Lemma subset_union_transl :
+    forall s sl sr,
+      subset s sl ->
+      subset s (set_union' sl sr).
+  Proof.
+    intros.
+    eapply subset_trans; [| apply subset_union_comm ].
+    apply subset_union_transr; auto.
+  Qed.
+
+
+  Lemma set_union_subset_cong :
+    forall sl sr sl' sr',
+      subset sl sl' -> subset sr sr' -> subset (set_union' sl sr) (set_union' sl' sr').
+  Proof.
+    induction sr.
+    intros.
+    apply subset_trans with (s2 := sl).
+    apply set_union_unitr.
+    apply subset_union_transl; auto.
+
+    intros sl' sr' Hsubl Hsubr.
+    simpl.
+    apply subset_trans with (s2 := (a :: set_union' sl sr)).
+    apply set_subset_weaken.
+    apply set_eq_symm.
+    apply set_add_cons_eq.
+    simpl.
+    split.
+    apply elem_union.
+    destruct Hsubr; auto.
+    apply IHsr; auto.
+    eapply subset_trans.
+    eapply subset_consr.
+    apply subset_refl.
+    apply Hsubr.
+  Qed.
+
+  Lemma set_union_cong : forall sl sr sl' sr',
+                           set_eq sl sl' -> set_eq sr sr' -> set_eq (set_union' sl sr) (set_union' sl' sr').
+  Proof.
+    intros sl sr sl' sr' Hl Hr.
+    destruct Hl as [Hl Hl'].
+    destruct Hr as [Hr Hr'].
+    split; apply set_union_subset_cong; auto.
+  Qed.
+
+
+  Lemma set_subset_add : forall x s1 s2, subset s1 s2 -> subset s1 (set_add' x s2).
+  Proof.
+    intros x s1 s2 Hsub.
+    eapply subset_trans; [| apply set_add_cons_subset; apply subset_refl ].
+    apply subset_consr; auto.
+  Qed.
+
+  Theorem set_eq_app_cons_comm s1 s2 a : set_eq (a :: (s1 ++ s2)) (s1 ++ a :: s2).
+  Proof.
+    induction s1.
+    apply set_eq_refl.
+    rewrite <-app_comm_cons.
+    eapply set_eq_trans.
+    apply set_eq_cons_swap.
+    apply set_eq_refl.
+    replace ((a0 :: s1) ++ a :: s2) with (a0 :: (s1 ++ a :: s2)) by apply app_comm_cons.
+    apply set_eq_cons_cons; auto.
+  Qed.
+
+  Theorem set_union_app_eq : forall s1 s2, set_eq (set_union' s1 s2) (s1 ++ s2).
+  Proof.
+    induction s2.
+    simpl.
+    rewrite app_nil_r.
+    apply set_eq_refl.
+
+    simpl.
+    eapply set_eq_trans.
+    apply set_eq_symm.
+    apply set_add_cons_eq.
+    eapply set_eq_trans; [|   apply set_eq_app_cons_comm].
+    apply set_eq_cons_cons; auto.
+  Qed.
+
+  Theorem set_union_app_eq_gen : forall s1 s2 s3 s4,
+                                   set_eq s1 s3 ->
+                                   set_eq s2 s4 ->
+                                   set_eq (set_union' s1 s2) (s3 ++ s4).
+  Proof.
+    intros s1 s2 s3 s4 H13 H24.
+    eapply set_eq_trans; [| apply set_union_app_eq].
+    apply set_union_cong; auto.
+  Qed.
+
+
+  Theorem subset_union_both s sl sr
+  : subset sl s -> subset sr s -> subset (set_union' sl sr) s.
+  Proof.
+    intros Hls Hrs.
+    apply subset_In_def.
+    intros x Hin.
+    destruct (set_union_elim eq_nat_dec x sl sr).
+    apply Hin.
+    apply In_subset_def with sl; auto.
+    apply In_subset_def with sr; auto.
+  Qed.
+
+  Theorem subset_union_eq : forall s1 s2, subset s1 s2 -> set_eq (set_union' s1 s2) s2.
+  Proof.
+    split; [| apply subset_union_transr; apply subset_refl ].
+    generalize dependent s2.
+    induction s1 as [| x s1].
+    intros s1 Hsubnil.
+    apply subset_trans with (s2 := s1).
+    apply set_union_unitl; apply subset_refl.
+    apply subset_refl.
+
+    intros s2 Hsub.
+    apply subset_trans with (s2 := x :: (set_union' s1 s2)).
+    apply subset_trans with (s2 := (x :: s1 ++ s2)).
+    apply set_union_app_eq.
+    apply set_subset_weaken.
+    apply set_eq_cons_cons.
+    apply set_eq_symm.
+    apply set_union_app_eq.
+
+    simpl.
+    unfold subset in Hsub; fold subset in Hsub.
+    destruct Hsub.
+    split; auto.
+  Qed.
+
+  Theorem set_union_assoc s1 s2 s3
+  : set_eq (set_union' (set_union' s1 s2) s3)
+           (set_union' s1 (set_union' s2 s3)).
+  Proof.
+    apply set_eq_trans with (s2 := ((s1 ++ s2) ++ s3)).
+    apply set_union_app_eq_gen.
+    apply set_union_app_eq.
+    apply set_eq_refl.
+    rewrite <-app_assoc.
+    apply set_eq_symm.
+    apply set_union_app_eq_gen.
+    apply set_eq_refl.
+    apply set_union_app_eq.
+  Qed.
+
+  Example set_eq_test : (set_eq (set_add' 1 (set_add' 0 empty_set'))
+                                (set_add' 0 (set_add' 1 empty_set'))).
+  Proof.
+    compute.
+    tauto.
+  Qed.
+
+  Lemma subset_app : forall s1 s2 s3, subset s1 s2 -> subset s1 (s2 ++ s3).
+  Proof.
+    induction s1; auto.
+    induction s2.
+
+    intros s3 H.
+    inversion H.
+    inversion H0.
+
+    intros s3.
+    simpl.
+    rewrite app_comm_cons.
+    intros H.
+    destruct H.
+    destruct H.
     subst.
-    erewrite (IHe _ _ _ _ _ H3 H11) in *.
-    erewrite (H _ _ _ _ _ _ H7 H15) in *.
-    erewrite (Pairing_from_fun _ _ _ _ H2 H10) in *.
+    split.
+    left; auto.
+    apply IHs1; auto.
+
+    split.
+    right.
+    unfold set_In.
+    apply in_or_app.
+    left; auto.
+
+    apply IHs1; auto.
+  Qed.
+  Lemma subset_rev : forall s, subset s (rev s).
+  Proof.
+    induction s; auto.
+    constructor.
+    rewrite <-in_rev.
+    constructor; auto.
+    replace (a :: s) with ((a :: nil) ++ s).
+    rewrite rev_app_distr.
+    apply subset_app; auto.
+
     auto.
-
-  (* E_Sum Left *)
-  - inversion H10; subst.
-    erewrite (IHe1 _ _ _ _ _ H5 H12).
-    auto.
-
-  (* E_Sum Right *)
-  - inversion H10; subst.
-    erewrite (IHe2 _ _ _ _ _ H5 H12).
-    auto.
-
-  (* E_Trace *)
-  - apply IHe with (x := x) (t1 := _t) (t2 := _t0); assumption.
-Qed.
-
-Lemma even_fun:
-  forall x y,
-    2 * x = 2 * y ->
-    x = y.
-Proof.
-  induction x as [|x]; intros; nliamega.
-Qed.
-
-Lemma odd_neq_even:
-  forall x y,
-    2 * x = 2 * y + 1 ->
-    False.
-Proof.
-  induction x as [|x]; intros; nliamega.
-Qed.
-
-Lemma odd_fun:
-  forall x y,
-    2 * x + 1 = 2 * y + 1 ->
-    x = y.
-Proof.
-  induction x as [|x]; intros; nliamega.
-Qed.
-
-Theorem Enumerates_from_fun :
-  forall e n x1 x2 t1 t2,
-    Enumerates e n x1 t1 ->
-    Enumerates e n x2 t2 ->
-    x1 = x2 /\ t1 = t2.
-Proof.
-  induction e; intros x n1 n2 t1 t2 E1 E2; inversion E1; inversion E2; eauto; subst; try congruence.
-
-  (* E_Pair *)
-  - erewrite (Pairing_to_l_fun _ _ _ _ _ H1 H9) in *.
-    erewrite (Pairing_to_r_fun _ _ _ _ _ H1 H9) in *.
-    destruct (IHe1 _ _ _ _ _ H2 H10); subst.
-    destruct (IHe2 _ _ _ _ _ H6 H14); subst.
-    auto.
-
-  (* E_Map *)
-  - destruct (IHe _ _ _ _ _ H5 H12); subst.
-    erewrite (Bijects_fun_left _ _ _ _ _ _ H1 H8) in *.
-    auto.
-
-  (* E_Dep *)
-  - erewrite (Pairing_to_l_fun _ _ _ _ _ H2 H10) in *.
-    erewrite (Pairing_to_r_fun _ _ _ _ _ H2 H10) in *.
-    destruct (IHe _ _ _ _ _ H3 H11); subst.
-    destruct (H _ _ _ _ _ _ H7 H15); subst.
-    auto.
-
-  (* E_Sum Left *)
-  - erewrite (even_fun _ _ H8) in *.
-    destruct (IHe1 _ _ _ _ _ H5 H12); subst.
-    auto.
-
-
-  (* E_Sum Left & Right *)
-  - apply odd_neq_even in H8. contradiction.
-
-  (* E_Sum Right & Left *)
-  - subst. symmetry in H8. apply odd_neq_even in H8. contradiction.
-
-  (* E_Sum Right *)
-  - erewrite (odd_fun _ _ H8) in *.
-    destruct (IHe2 _ _ _ _ _ H5 H12); subst.
-    auto.
-
-  (* E_Trace *)
-  - destruct (IHe _ _ _ _ _ H4 H10); subst.
-    auto.
-Qed.
-
-(* Map/Trace compatibility lemmas *)
-Lemma Enumerates_to_dec_Map :
-  forall b e x,
-    (forall x,
-      { nt: nat * Trace | let (n, t) := nt in Enumerates e n x t }
-      + { forall n t, ~ Enumerates e n x t }) ->
-    { nt : nat * Trace | let (n, t) := nt in Enumerates (E_Map b e) n x t }
-    + { forall n t, ~ Enumerates (E_Map b e) n x t }.
-Proof.
-  intros b e x IHe.
-  destruct (Bijects_to_dec _ _ b x) as [y B].
-  destruct (IHe y) as [[nt IHE] | NIH].
-
-  left. exists nt. destruct nt. eauto.
-
-  right. intros n t E.
-  inversion E. subst n0 x0 t0 inner bi.
-  rename H1 into B'. rename H5 into IHE.
-  erewrite (Bijects_fun_right _ _ _ _ _ _ B B') in *.
-  eapply NIH. apply IHE.
-Defined.
-Hint Resolve Enumerates_to_dec_Map.
-
-Lemma Enumerates_to_dec_Trace :
-  forall tg e x,
-    (forall x,
-      { nt: nat * Trace | let (n, t) := nt in Enumerates e n x t }
-      + { forall n t, ~ Enumerates e n x t }) ->
-    { nt : nat * Trace | let (n, t) := nt in Enumerates (E_Trace tg e) n x t }
-    + { forall n t, ~ Enumerates (E_Trace tg e) n x t }.
-Proof.
-  intros tg e x IHe.
-  destruct (IHe x) as [[[n t] IHE] | NIH].
-
-  left.
-  exists (n, trace_one n tg); eauto.
-
-  right.
-  intros n t E.
-  inversion E; eapply NIH; eauto.
-Defined.
-Hint Resolve Enumerates_to_dec_Trace.
-
-
-Definition Enumerates_to_dec:
-  forall e x,
-    { nt : nat * Trace | let (n, t) := nt in Enumerates e n x t } + { forall n t, ~ Enumerates e n x t }.
-Proof.
-  induction e; destruct x; eauto;
-    try ( right; intros _n _t E; inversion E; fail ).
-
-  (* E_Nat *)
-  - left; exists (n, trace_zero); constructor.
-
-  (* E_Pair *)
-  - rename x1 into lx. rename x2 into rx.
-    rename e1 into l. rename e2 into r.
-    destruct (IHe1 lx) as [[[ln lt] EL] | LF].
-    destruct (IHe2 rx) as [[[rn rt] ER] | RF].
-    left.
-    destruct (Pairing_to_dec ln rn) as [n P].
-    exists (n, trace_plus lt rt).
-    eauto.
-
-    right. intros _n _t E; inversion E; subst.
-    eapply RF; eauto.
-
-    right. intros _n _t E; inversion E; subst.
-    eapply LF; eauto.
-
-  (* E_Dep *)
-  - destruct (IHe x1) as [[[ln lt] EL] | LF].
-    destruct (X x1 x2) as [[[rn rt] ER] | RF].
-    left.
-    destruct (Pairing_to_dec ln rn) as [n P].
-    exists (n, trace_plus lt rt).
-    eauto.
-
-    right. intros _n _t E; inversion E; subst.
-    eapply RF; eauto.
-
-    right. intros _n _t E; inversion E; subst.
-    eapply LF; eauto.
-
-  (* E_Sum Left *)
-  - destruct (IHe1 x) as [[[ln lt] EL] | LF].
-    left. exists (2 * ln, lt). eauto.
-
-    right. intros _n _t E. inversion E; subst.
-    eapply LF; eauto.
-
-  (* E_Sum Right *)
-  - destruct (IHe2 x) as [[[rn rt] ER] | RF].
-    left. exists (2 * rn + 1, rt). eauto.
-
-    right. intros _n _t E. inversion E; subst.
-    eapply RF; eauto.
-Defined.
-
-Lemma even_SS :
-  forall n,
-    { l | n = 2 * l } -> { m | S (S n) = 2 * m }.
-Proof.
-  intros n P.
-  destruct P.
-  exists ((S x)).
-  nliamega.
-Defined.
-
-Lemma odd_SS :
-  forall n,
-    { r | n = 2 * r + 1 } -> { m | S (S n) = 2 * m + 1 }.
-Proof.
-  intros n P.
-  destruct P.
-  exists ((S x)).
-  nliamega.
-Defined.
-
-Fixpoint even_odd_eq_dec n : { l | n = 2 * l } + { r | n = 2 * r + 1 }.
-Proof.
-  refine (match n with
-            | 0 => _
-            | S 0 => _
-            | S (S n') => _
-          end).
-  left;  exists 0; auto.
-  right; exists 0; auto.
-
-  clear n0.
-  destruct (even_odd_eq_dec n').
-  left; apply even_SS; assumption.
-  right; apply odd_SS; assumption.
-Defined.
-
-Definition Enumerates_from_dec:
-  forall e n,
-    { xt : Value * Trace | let (x, t) := xt in Enumerates e n x t }.
-Proof.
-  induction e; intros n; eauto.
-
-  (* E_Nat *)
-  - exists (V_Nat n, trace_zero); eauto.
-
-  (* E_pair *)
-  - rename e1 into l. rename e2 into r.
-    remember (Pairing_from n) as PF.
-    destruct PF as [ln rn].
-    destruct (IHe1 ln) as [[lx lt] EL].
-    destruct (IHe2 rn) as [[rx rt] ER].
-    exists (V_Pair lx rx, trace_plus lt rt).
-    eauto.
-
-  (* E_Map *)
-  - destruct (IHe n) as [[x t] IHE].
-    destruct (Bijects_from_dec _ _ b x) as [y B].
-    exists (y, t). eauto.
-
-  (* E_Dep *)
-  - rename e into l. rename e0 into f.
-    remember (Pairing_from n) as PF.
-    destruct PF as [ln rn].
-    destruct (IHe ln) as [[lx lt] EL].
-    destruct (X lx rn) as [[rx rt] ER].
-    exists (V_Pair lx rx, trace_plus lt rt). eauto.
-
-  (* E_Sum *)
-  - destruct (even_odd_dec n) as [Hev | Hodd].
-    apply even_double in Hev.
-    destruct (IHe1 (div2 n)) as [[lx lt] EL].
-    exists (V_Sum_Left lx, lt).
-    rewrite double_twice in Hev.
-    eauto.
-
-    apply odd_double in Hodd.
-    destruct (IHe2 (div2 n)) as [[rx rt] ER].
-    exists (V_Sum_Right rx, rt).
-    rewrite double_twice in Hodd.
-    replace (S (2 * div2 n)) with (2 * div2 n + 1) in Hodd by nliamega.
-    eauto.
-
-  (* E_Trace *)
-  - rename t into tg.
-    destruct (IHe n) as [[x _t] E].
-    exists (x, trace_one n tg).
-    eauto.
-Defined.
-
-Definition Trace_on (e : Enum) (n : nat) : Trace :=
-  let (nt, _) := (Enumerates_from_dec e n) in snd nt.
-
-Fixpoint Trace_lt (e : Enum) n : Trace :=
-  match n with
-    | 0 => trace_zero
-    | S n' => trace_plus (Trace_on e n') (Trace_lt e n')
-  end.
-
-Fixpoint Trace_from_to e lo hi : Trace :=
-  if le_lt_dec hi lo
-  then trace_zero
-  else match hi with
-         | 0 => trace_zero
-         | S hi' => trace_plus (Trace_on e hi') (Trace_from_to e lo hi')
-       end.
-
-Fixpoint subset (s1 s2 : set nat) :=
-  match s1 with
-    | nil => True
-    | x :: more =>
-      set_In x s2 /\ subset more s2
-  end.
-Hint Unfold subset.
-
-Theorem subset_nil : forall s, subset nil s.
-Proof.
-  auto.
-Qed.
-
-Theorem subset_nil_nil : forall s, subset s nil -> s = nil.
-Proof.
-  induction s.
-  auto.
-  intros contra.
-  unfold subset in contra.
-  destruct contra.
-  inversion H.
-Qed.
-
-Definition set_eq s1 s2 := subset s1 s2 /\ subset s2 s1.
-Hint Unfold set_eq.
-
-Lemma subset_consr s1 s2 n : subset s1 s2 -> subset s1 (cons n s2).
-Proof.
-  generalize dependent s2.
-  generalize dependent n.
-  induction s1.
-  constructor.
-
-  intros n s2 H.
-  unfold subset.
-  unfold subset in H.
-  destruct H.
-  fold subset in *.
-
-  split.
-  constructor 2; auto.
-  apply IHs1; auto.
-Defined.
-
-Definition subset_dec s1 s2 : { subset s1 s2 } + { ~ (subset s1 s2) }.
-Proof.
-  generalize dependent s2.
-  induction s1.
-  left; auto.
-
-  intros s2.
-  destruct (In_dec eq_nat_dec a s2).
-
-  destruct (IHs1 s2).
-  left; constructor; auto.
-
-  right.
-  unfold subset; fold subset.
-  intros H; destruct H; contradiction.
-
-  right.
-  intros H; destruct H; contradiction.
-Defined.
-
-Definition subset_nn s1 s2 : ~~(subset s1 s2) -> subset s1 s2.
-Proof.
-  destruct (subset_dec s1 s2); tauto.
-Qed.
-
-Definition set_eq_dec s1 s2 : { set_eq s1 s2 } + { ~ (set_eq s1 s2) }.
-Proof.
-  destruct (subset_dec s1 s2).
-  destruct (subset_dec s2 s1).
-  left; auto.
-  right; intros contra; destruct contra; apply n; auto.
-  right; intros contra; destruct contra; apply n; auto.
-Qed.
-
-Theorem subset_refl s : subset s s.
-Proof.
-  induction s; unfold subset; auto.
-  fold subset.
-  split.
-  constructor 1; auto.
-  apply subset_consr; auto.
-Qed.
-
-Theorem set_eq_refl s : set_eq s s.
-Proof.
-  split; apply subset_refl.
-Qed.
-
-Theorem subset_In : forall x s s', set_In x s -> subset s s' -> set_In x s'.
-Proof.
-  intros x s.
-  generalize dependent x.
-  induction s as [| x s].
-  intros y s contra.
-  inversion contra.
-
-  intros y s' Hyinxs Hsub.
-  destruct Hsub as [Hxins' Hsub].
-  destruct Hyinxs; subst; auto.
-Qed.
-
-Theorem subset_In_def s s' : (forall x, set_In x s -> set_In x s') -> subset s s'.
-Proof.
-  generalize dependent s'.
-  induction s.
-  intros; apply subset_nil.
-  split.
-  apply H; auto.
-  constructor; auto.
-  apply IHs.
-  intros x Hins.
-  apply H.
-  constructor 2; auto.
-Qed.
-
-Theorem In_subset_def s s' : subset s s' -> (forall x, set_In x s -> set_In x s').
-Proof.
-  generalize dependent s'.
-  induction s.
-  intros s' _ x contra.
-  inversion contra.
-
-  intros s' Hsub x Hin.
-  destruct Hin.
-  destruct Hsub; subst.
-  auto.
-
-  apply IHs.
-  destruct Hsub; subst; auto.
-  auto.
-Qed.
-
-Hint Resolve subset_In_def In_subset_def.
-Theorem subset_In_equiv s s' : subset s s' <-> (forall x, set_In x s -> set_In x s').
-Proof.
-  split; eauto.
-Qed.
-
-Lemma set_subset_weaken : forall s1 s2, set_eq s1 s2 -> subset s1 s2.
-Proof.
-  unfold set_eq.
-  tauto.
-Qed.
-
-Theorem not_subset_In_def s s' x : set_In x s -> ~(set_In x s') -> ~ subset s s'.
-Proof.
-  intros; eauto.
-Qed.
-
-Lemma subset_trans : forall s1 s2 s3, subset s1 s2 -> subset s2 s3 -> subset s1 s3.
-Proof.
-  intros s1.
-  induction s1 as [| x s1].
-  intros; apply subset_nil.
-  induction s2 as [| y s2].
-  intros s3 contra.
-  inversion contra.
-  inversion H.
-
-  intros s3 Hxy12 Hy23.
-  unfold subset; fold subset.
-  destruct Hxy12 as [Hxy2 H1y2].
-  split.
-
-  eapply subset_In.
-  apply Hxy2.
-  auto.
-  apply IHs1 with (s2 := (y :: s2)); auto.
-Qed.
-
-
-Lemma set_eq_trans : forall s1 s2 s3, set_eq s1 s2 -> set_eq s2 s3 -> set_eq s1 s3.
-Proof.
-  unfold set_eq.
-  intros s1 s2 s3 H1 H2; destruct H1; destruct H2.
-  split; eapply subset_trans; eauto.
-Qed.
-
-Lemma set_eq_symm : forall s1 s2, set_eq s1 s2 -> set_eq s2 s1.
-Proof.
-  intros s1 s2 H; inversion H; split; auto.
-Qed.
-
-(* Theorem set_union_or : forall s1 s2, subset s1 (set_union' s1 s2). *)
-
-Lemma set_add_subset : forall x s1 s2, set_In x s2 -> subset s1 s2 -> subset (set_add' x s1) s2.
-Proof.
-
-  intros y s1.
-  induction s1 as [| x s1].
-  simpl; auto.
-  intros s2 Hy2 Hsub.
-  unfold set_add', set_add.
-  destruct (eq_nat_dec y x); subst; auto.
-  fold set_add.
-  unfold subset.
-  split; auto.
-  destruct Hsub; auto.
-  fold subset.
-  apply IHs1; auto.
-  destruct Hsub; auto.
-Qed.
-
-Lemma subset_cons_swap : forall x y s1 s2, subset s1 s2 -> subset (x :: y :: s1) (y :: x :: s2).
-Proof.
-  intros x y s1 s2.
-  destruct (eq_nat_dec x y).
-  simpl; subst.
-  split.
-  tauto.
-  split.
-  tauto.
-  apply subset_consr.
-  apply subset_consr.
-  assumption.
-
-  simpl.
-  split.
-  tauto.
-  split.
-  tauto.
-  apply subset_consr. apply subset_consr.
-  assumption.
-Qed.
-
-Lemma set_eq_cons_swap : forall x y s1 s2, set_eq s1 s2 -> set_eq (x :: y :: s1) (y :: x :: s2).
-Proof.
-  split; destruct H; apply subset_cons_swap; auto.
-Qed.
-
-Lemma set_cons_cons_subset : forall x s1 s2, subset s1 s2 -> subset (x :: s1) (x :: s2).
-Proof.
-  intros x s1 s2 Hsub.
-  unfold subset. fold subset.
-  split.
-  constructor; auto.
-  apply subset_consr; auto.
-Qed.
-
-Lemma set_eq_cons_cons x s1 s2 : set_eq s1 s2 -> set_eq (x :: s1) (x :: s2).
-Proof.
-  intros H.
-  destruct H.
-  split; apply set_cons_cons_subset; auto.
-Qed.
-
-Lemma set_add_cons_eq : forall x s, set_eq (x :: s) (set_add' x s).
-Proof.
-  split.
-  generalize dependent x.
-  induction s as [| y s].
-  compute; tauto.
-  intros x.
-  simpl.
-  destruct (eq_nat_dec x y); subst.
-  split.
-  constructor; auto.
-  split.
-  constructor; auto.
-  apply subset_consr.
-  apply subset_refl.
-
-  split.
-  destruct (IHs x).
-  apply in_cons. apply H.
-  split.
-  constructor; auto.
-  apply subset_trans with (s2:= (x :: s)).
-  apply subset_consr; auto.
-
-  apply subset_trans with (s2 := (set_add' x s)).
-  apply IHs.
-  apply subset_consr.
-  apply subset_refl.
-
-  generalize dependent x.
-  induction s as [| y s].
-  compute; tauto.
-  intros x.
-  simpl.
-  destruct (eq_nat_dec x y).
-  apply subset_consr.
-  apply subset_refl.
-  apply subset_trans with (y :: x :: s).
-  apply set_cons_cons_subset.
-  apply IHs.
-  apply subset_cons_swap.
-  apply subset_refl.
-Qed.
-
-Lemma set_add_cons_subset : forall x s1 s2, subset s1 s2 -> subset (x :: s1) (set_add' x s2).
-Proof.
-  intros x s1 s2 Hsub.
-  apply subset_trans with (s2 := (x :: s2)).
-  apply set_cons_cons_subset; auto.
-  apply set_subset_weaken.
-  apply set_add_cons_eq.
-Qed.
-
-Lemma set_union_unitl : forall s, set_eq (set_union' empty_set' s) s.
-Proof.
-  split.
-  induction s.
-  apply subset_refl.
-
-  unfold set_union', set_union in *.
-  replace (((fix set_union (x y : set nat) {struct y} :
-          set nat :=
-            match y with
-            | nil => x
-            | a1 :: y1 => set_add eq_nat_dec a1 (set_union x y1)
-            end) empty_set' s
-           )) with (set_union' empty_set' s) in * by auto.
-  fold set_add'.
-  apply set_add_subset; auto.
-  constructor; auto.
-  apply subset_consr; auto.
-
-  induction s; auto.
-  unfold set_union', set_union.
-  fold set_union.
-  apply set_add_cons_subset; auto.
-Qed.
-
-Lemma set_union_unitr : forall s, set_eq (set_union' s empty_set') s.
-Proof.
-  apply set_eq_refl.
-Qed.
-
-Lemma elem_union :
-  forall s x,
-    set_In x s -> forall s', set_In x (set_union' s' s).
-Proof.
-  induction s.
-  intros H contra.
-  inversion contra.
-
-  intros x Hin s'.
-  simpl.
-  assert (set_In x (a :: (set_union' s' s))).
-  destruct Hin.
-  constructor; auto.
-  eapply In_subset_def.
-  apply subset_consr.
-  apply subset_refl.
-  apply IHs; auto.
-  eapply In_subset_def.
-  apply set_add_cons_subset.
-  apply subset_refl.
-  auto.
-Qed.
-
-Lemma subset_union_cons : forall x s1 s2, subset (set_union' (x::s1) s2) (x :: (set_union' s1 s2)).
-  induction s2.
-  simpl; split.
-  tauto.
-  apply subset_consr; apply subset_refl.
-  simpl.
-  eapply subset_trans.
-  apply set_add_cons_eq.
-  apply subset_trans with (s2 := (x :: a :: (set_union' s1 s2))).
-  eapply subset_trans.
-  apply set_cons_cons_subset.
-  apply IHs2.
-  apply subset_cons_swap.
-  apply subset_refl.
-  apply set_cons_cons_subset.
-  apply set_add_cons_eq.
-Qed.
-
-Theorem subset_union_comm : forall s1 s2, subset (set_union' s1 s2) (set_union' s2 s1).
-Proof.
-  induction s1.
-  intros.
-  apply subset_trans with (s2 := s2).
-  apply set_union_unitl.
-  apply set_union_unitr.
-
-  intros s2.
-  simpl.
-  eapply subset_trans.
-  apply subset_union_cons.
-  apply set_add_cons_subset.
-  apply IHs1.
-Qed.
-
-Theorem set_eq_union_comm : forall s1 s2, set_eq (set_union' s1 s2) (set_union' s2 s1).
-Proof.
-  intros s1 s2.
-  split; apply subset_union_comm.
-Qed.
-
-Lemma subset_union_transr :
-  forall s sl sr,
-    subset s sr ->
-    subset s (set_union' sl sr).
-Proof.
-  intros.
-  apply subset_In_def.
-  intros x Hin.
-  apply elem_union.
-  eapply In_subset_def.
-  apply H.
-  auto.
-Qed.
-
-Lemma subset_union_transl :
-  forall s sl sr,
-    subset s sl ->
-    subset s (set_union' sl sr).
-Proof.
-  intros.
-  eapply subset_trans; [| apply subset_union_comm ].
-  apply subset_union_transr; auto.
-Qed.
-
-
-Lemma set_union_subset_cong :
-  forall sl sr sl' sr',
-    subset sl sl' -> subset sr sr' -> subset (set_union' sl sr) (set_union' sl' sr').
-Proof.
-  induction sr.
-  intros.
-  apply subset_trans with (s2 := sl).
-  apply set_union_unitr.
-  apply subset_union_transl; auto.
-
-  intros sl' sr' Hsubl Hsubr.
-  simpl.
-  apply subset_trans with (s2 := (a :: set_union' sl sr)).
-  apply set_subset_weaken.
-  apply set_eq_symm.
-  apply set_add_cons_eq.
-  simpl.
-  split.
-  apply elem_union.
-  destruct Hsubr; auto.
-  apply IHsr; auto.
-  eapply subset_trans.
-  eapply subset_consr.
-  apply subset_refl.
-  apply Hsubr.
-Qed.
-
-Lemma set_union_cong : forall sl sr sl' sr',
-                         set_eq sl sl' -> set_eq sr sr' -> set_eq (set_union' sl sr) (set_union' sl' sr').
-Proof.
-  intros sl sr sl' sr' Hl Hr.
-  destruct Hl as [Hl Hl'].
-  destruct Hr as [Hr Hr'].
-  split; apply set_union_subset_cong; auto.
-Qed.
-
-
-Lemma set_subset_add : forall x s1 s2, subset s1 s2 -> subset s1 (set_add' x s2).
-Proof.
-  intros x s1 s2 Hsub.
-  eapply subset_trans; [| apply set_add_cons_subset; apply subset_refl ].
-  apply subset_consr; auto.
-Qed.
-
-Theorem set_eq_app_cons_comm s1 s2 a : set_eq (a :: (s1 ++ s2)) (s1 ++ a :: s2).
-Proof.
-  induction s1.
-  apply set_eq_refl.
-  rewrite <-app_comm_cons.
-  eapply set_eq_trans.
-  apply set_eq_cons_swap.
-  apply set_eq_refl.
-  replace ((a0 :: s1) ++ a :: s2) with (a0 :: (s1 ++ a :: s2)) by apply app_comm_cons.
-  apply set_eq_cons_cons; auto.
-Qed.
-
-Theorem set_union_app_eq : forall s1 s2, set_eq (set_union' s1 s2) (s1 ++ s2).
-Proof.
-  induction s2.
-  simpl.
-  rewrite app_nil_r.
-  apply set_eq_refl.
-
-  simpl.
-  eapply set_eq_trans.
-  apply set_eq_symm.
-  apply set_add_cons_eq.
-  eapply set_eq_trans; [|   apply set_eq_app_cons_comm].
-  apply set_eq_cons_cons; auto.
-Qed.
-
-Theorem set_union_app_eq_gen : forall s1 s2 s3 s4,
-                                 set_eq s1 s3 ->
-                                 set_eq s2 s4 ->
-                                 set_eq (set_union' s1 s2) (s3 ++ s4).
-Proof.
-  intros s1 s2 s3 s4 H13 H24.
-  eapply set_eq_trans; [| apply set_union_app_eq].
-  apply set_union_cong; auto.
-Qed.
-
-
-Theorem subset_union_both s sl sr
-: subset sl s -> subset sr s -> subset (set_union' sl sr) s.
-Proof.
-  intros Hls Hrs.
-  apply subset_In_def.
-  intros x Hin.
-  destruct (set_union_elim eq_nat_dec x sl sr).
-  apply Hin.
-  apply In_subset_def with sl; auto.
-  apply In_subset_def with sr; auto.
-Qed.
-
-Theorem subset_union_eq : forall s1 s2, subset s1 s2 -> set_eq (set_union' s1 s2) s2.
-Proof.
-  split; [| apply subset_union_transr; apply subset_refl ].
-  generalize dependent s2.
-  induction s1 as [| x s1].
-  intros s1 Hsubnil.
-  apply subset_trans with (s2 := s1).
-  apply set_union_unitl; apply subset_refl.
-  apply subset_refl.
-
-  intros s2 Hsub.
-  apply subset_trans with (s2 := x :: (set_union' s1 s2)).
-  apply subset_trans with (s2 := (x :: s1 ++ s2)).
-  apply set_union_app_eq.
-  apply set_subset_weaken.
-  apply set_eq_cons_cons.
-  apply set_eq_symm.
-  apply set_union_app_eq.
-
-  simpl.
-  unfold subset in Hsub; fold subset in Hsub.
-  destruct Hsub.
-  split; auto.
-Qed.
-
-Theorem set_union_assoc s1 s2 s3
-: set_eq (set_union' (set_union' s1 s2) s3)
-         (set_union' s1 (set_union' s2 s3)).
-Proof.
-  apply set_eq_trans with (s2 := ((s1 ++ s2) ++ s3)).
-  apply set_union_app_eq_gen.
-  apply set_union_app_eq.
-  apply set_eq_refl.
-  rewrite <-app_assoc.
-  apply set_eq_symm.
-  apply set_union_app_eq_gen.
-  apply set_eq_refl.
-  apply set_union_app_eq.
-Qed.
-
-Example set_eq_test : (set_eq (set_add' 1 (set_add' 0 empty_set'))
-                              (set_add' 0 (set_add' 1 empty_set'))).
-Proof.
-  compute.
-  tauto.
-Qed.
-
-Definition Fair2 (k : Enum -> Enum -> Enum) :=
-  forall n,
-  exists equilibrium,
-    match Trace_lt (k (E_Trace zero E_Nat) (E_Trace one E_Nat)) equilibrium with
-      | Tracing l_uses r_uses _ _ =>
-        n < equilibrium /\ set_eq  l_uses r_uses
+  Qed.
+
+  Lemma set_eq_rev : forall s, set_eq s (rev s).
+  Proof.
+    split; try apply subset_rev.
+    rewrite <-rev_involutive.
+    apply subset_rev.
+  Qed.
+  
+  Fixpoint z_to_n n : set nat :=
+    match n with
+      | 0 => empty_set'
+      | S n' => set_add' n' (z_to_n n')
     end.
 
-Definition Fair3 (k : Enum -> Enum -> Enum -> Enum) :=
-  forall n,
-  exists equilibrium,
-    match Trace_lt (k (E_Trace zero E_Nat) (E_Trace one E_Nat) (E_Trace two E_Nat)) equilibrium with
-      | Tracing z_uses o_uses t_uses _ =>
-        n < equilibrium /\ set_eq z_uses o_uses /\ set_eq o_uses t_uses
-    end.
+  Definition n_to_z n : set nat := rev (z_to_n n).
 
-Definition Fair4 (k : Enum -> Enum -> Enum -> Enum -> Enum) :=
-  forall n,
-  exists equilibrium,
-    match Trace_lt (k (E_Trace zero E_Nat) (E_Trace one E_Nat) (E_Trace two E_Nat) (E_Trace three E_Nat)) equilibrium with
-      | Tracing z_uses o_uses tw_uses th_uses =>
-        n < equilibrium /\ set_eq z_uses o_uses /\ set_eq o_uses tw_uses /\ set_eq tw_uses th_uses
-    end.
+  Theorem z_to_n_correct n x
+  : set_In x (z_to_n n) <-> x < n.
+  Proof.
+    generalize dependent x.
+    induction n.
 
-Lemma Sum_Parity_Trace :
-  forall n,
-    Trace_on (E_Sum (E_Trace zero E_Nat) (E_Trace one E_Nat)) n
-    = trace_one (div2 n)
-                (if even_odd_dec n
-                 then zero
-                 else one).
-Proof.
-  intros n.
-  remember (even_odd_dec n) as mH.
-  unfold Trace_on; simpl.
-  destruct mH; rewrite <-HeqmH; auto.
-Qed.
+    intros x; compute; split; [apply False_ind | intros contra; inversion contra].
+    intros x.
+    destruct (eq_nat_dec x n).
+    simpl.
+    subst.
+    split; [nliamega|].
+    intros _.
+    apply set_add_intro2; auto.
 
-Fixpoint z_to_n n : set nat :=
-  match n with
-    | 0 => empty_set'
-    | S n' => set_add' n' (z_to_n n')
-  end.
+    split.
+    simpl.
+    intros H.
+    assert (set_In x (z_to_n n)).
+    apply set_add_elim2 with (b := n) (Aeq_dec := eq_nat_dec); auto.
+    assert (x < n).
+    apply IHn.
+    auto.
+    nliamega.
 
-Definition n_to_z n : set nat := rev (z_to_n n).
+    intros H.
+    simpl.
+    apply set_add_intro1.
+    apply IHn.
+    nliamega.
+  Qed.
 
-Lemma subset_app : forall s1 s2 s3, subset s1 s2 -> subset s1 (s2 ++ s3).
-Proof.
-  induction s1; auto.
-  induction s2.
+  Lemma z_to_n_nosubS m : ~ subset (z_to_n (S m)) (z_to_n m).
+  Proof.
+    intros H.
+    assert (set_In m (z_to_n m)).
+    eapply In_subset_def; eauto.
+    apply z_to_n_correct; nliamega.
+    rewrite z_to_n_correct in H0.
+    nliamega.
+  Qed.
 
-  intros s3 H.
-  inversion H.
-  inversion H0.
+  Lemma z_to_n_nosub' m n : ~ subset (z_to_n (S (m + n))) (z_to_n m).
+  Proof.
+    induction n.
+    replace (m + 0) with m by nliamega.
+    apply z_to_n_nosubS.
+    unfold z_to_n; fold z_to_n.
+    replace (m + S n) with (S (m + n)) by nliamega.
+    intros H.
+    apply IHn.
+    apply subset_In_def.
+    intros x.
+    rewrite z_to_n_correct.
+    intros Hlt.
+    assert (set_In x (set_add' (S (m + n)) (z_to_n (S (m + n))))).
+    replace (set_add' (S (m + n)) (z_to_n (S (m + n)))) with (z_to_n (S (S (m + n)))).
+    apply z_to_n_correct; nliamega.
+    trivial.
+    eapply In_subset_def.
+    apply H.
+    auto.
+  Qed.
 
-  intros s3.
-  simpl.
-  rewrite app_comm_cons.
-  intros H.
-  destruct H.
-  destruct H.
-  subst.
-  split.
-  left; auto.
-  apply IHs1; auto.
+  Lemma z_to_n_nosub m n : m < n -> ~ subset (z_to_n n) (z_to_n m).
+  Proof.
+    intros H1 H2.
+    destruct n; [nliamega|].
+    assert (n < m); [| nliamega].
+    apply z_to_n_correct.
+    eapply In_subset_def.
+    eapply subset_trans; eauto.
+    unfold set_In.
+    rewrite !z_to_n_correct; auto.
+  Qed.
 
-  split.
-  right.
-  unfold set_In.
-  apply in_or_app.
-  left; auto.
-
-  apply IHs1; auto.
-Qed.
-Lemma subset_rev : forall s, subset s (rev s).
-Proof.
-  induction s; auto.
-  constructor.
-  rewrite <-in_rev.
-  constructor; auto.
-  replace (a :: s) with ((a :: nil) ++ s).
-  rewrite rev_app_distr.
-  apply subset_app; auto.
-
-  auto.
-Qed.
-
-Lemma set_eq_rev : forall s, set_eq s (rev s).
-Proof.
-  split; try apply subset_rev.
-  rewrite <-rev_involutive.
-  apply subset_rev.
-Qed.
-
-Definition trace_eq (t1 t2 : Trace) : Prop :=
-  match (t1, t2) with
-    | (Tracing l0 l1 l2 l3, Tracing r0 r1 r2 r3) =>
-      set_eq l0 r0
-      /\ set_eq l1 r1
-      /\ set_eq l2 r2
-      /\ set_eq l3 r3
-  end.
-
-Definition sub_trace (t1 t2 : Trace) : Prop :=
-  match (t1, t2) with
-    | (Tracing l0 l1 l2 l3, Tracing r0 r1 r2 r3) =>
-      subset l0 r0
-      /\ subset l1 r1
-      /\ subset l2 r2
-      /\ subset l3 r3
-  end.
+End Sets.
+Hint Resolve set_eq_refl.
+Hint Resolve subset_refl.
 
 Ltac split4 := split; [| split; [| split]].
 Ltac destruct4 H := destruct H as [? [? [? ?]]].
+Section Traces.
+  Inductive Trace :=
+  | Tracing : set' -> set' -> set' -> set' -> Trace.
 
-Theorem sub_trace_refl t : sub_trace t t.
-Proof.
-  unfold sub_trace; destruct t; split4; apply subset_refl.
-Qed.
+  Definition trace_proj tg t :=
+    match t with
+      | Tracing t0 t1 t2 t3 =>
+        match tg with
+          | zero  => t0
+          | one   => t1
+          | two   => t2
+          | three => t3
+        end
+    end.
 
-Theorem sub_trace_trans t1 t2 t3 : sub_trace t1 t2 -> sub_trace t2 t3 -> sub_trace t1 t3.
-Proof.
-  unfold sub_trace; destruct t1, t2, t3.
-  intros H1 H2; destruct4 H1; destruct4 H2.
-  split4; eapply subset_trans; eauto.
-Qed.
 
-Theorem sub_trace_zero t : sub_trace trace_zero t.
-Proof. destruct t; compute; tauto. Qed.
+  Definition trace_zero : Trace := Tracing empty_set' empty_set' empty_set' empty_set'.
+  Definition trace_plus (t1 t2 : Trace) : Trace :=
+    match (t1, t2) with
+      | (Tracing l1 l2 l3 l4, Tracing r1 r2 r3 r4) =>
+        Tracing (set_union' l1 r1)
+                (set_union' l2 r2)
+                (set_union' l3 r3)
+                (set_union' l4 r4)
+    end.
 
-Theorem trace_eq_proj t1 t2 tg : trace_eq t1 t2 -> set_eq (trace_proj tg t1) (trace_proj tg t2).
-Proof.
-  unfold trace_eq, trace_proj; destruct t1; destruct t2; destruct tg; intuition.
-Qed.
+  Definition trace_one n t : Trace :=
+    match t with
+      | zero  => Tracing (set_add' n empty_set') empty_set' empty_set' empty_set'
+      | one   => Tracing empty_set' (set_add' n empty_set') empty_set' empty_set'
+      | two   => Tracing empty_set' empty_set' (set_add' n empty_set') empty_set'
+      | three => Tracing empty_set' empty_set' empty_set' (set_add' n empty_set')
+    end.
 
-Theorem sub_trace_proj t1 t2 tg : sub_trace t1 t2 -> subset (trace_proj tg t1) (trace_proj tg t2).
-Proof.
-  unfold sub_trace; destruct t1; destruct t2; destruct tg; intuition.
-Qed.
+  Definition trace_eq (t1 t2 : Trace) : Prop :=
+    match (t1, t2) with
+      | (Tracing l0 l1 l2 l3, Tracing r0 r1 r2 r3) =>
+        set_eq l0 r0
+        /\ set_eq l1 r1
+        /\ set_eq l2 r2
+        /\ set_eq l3 r3
+    end.
 
-Definition trace_eq' t1 t2 : Prop :=
-  sub_trace t1 t2 /\ sub_trace t2 t1.
-Theorem trace_eq'_weakenl t1 t2 : trace_eq' t1 t2 -> sub_trace t1 t2.
-Proof. unfold trace_eq'; intuition. Qed.
-Theorem trace_eq'_weakenr t1 t2 : trace_eq' t1 t2 -> sub_trace t2 t1.
-Proof. unfold trace_eq'; intuition. Qed.
-Theorem trace_eq_eq'_equiv t1 t2 : trace_eq t1 t2 <-> trace_eq' t1 t2.
-Proof.
-  unfold trace_eq, trace_eq', sub_trace, set_eq;
+  Definition sub_trace (t1 t2 : Trace) : Prop :=
+    match (t1, t2) with
+      | (Tracing l0 l1 l2 l3, Tracing r0 r1 r2 r3) =>
+        subset l0 r0
+        /\ subset l1 r1
+        /\ subset l2 r2
+        /\ subset l3 r3
+    end.
+
+  Theorem sub_trace_refl t : sub_trace t t.
+  Proof.
+    unfold sub_trace; destruct t; split4; apply subset_refl.
+  Qed.
+
+  Theorem sub_trace_trans t1 t2 t3 : sub_trace t1 t2 -> sub_trace t2 t3 -> sub_trace t1 t3.
+  Proof.
+    unfold sub_trace; destruct t1, t2, t3.
+    intros H1 H2; destruct4 H1; destruct4 H2.
+    split4; eapply subset_trans; eauto.
+  Qed.
+
+  Theorem sub_trace_zero t : sub_trace trace_zero t.
+  Proof. destruct t; compute; tauto. Qed.
+
+  Theorem trace_eq_proj t1 t2 tg : trace_eq t1 t2 -> set_eq (trace_proj tg t1) (trace_proj tg t2).
+  Proof.
+    unfold trace_eq, trace_proj; destruct t1; destruct t2; destruct tg; intuition.
+  Qed.
+
+  Theorem sub_trace_proj t1 t2 tg : sub_trace t1 t2 -> subset (trace_proj tg t1) (trace_proj tg t2).
+  Proof.
+    unfold sub_trace; destruct t1; destruct t2; destruct tg; intuition.
+  Qed.
+
+  Definition trace_eq' t1 t2 : Prop :=
+    sub_trace t1 t2 /\ sub_trace t2 t1.
+  Theorem trace_eq'_weakenl t1 t2 : trace_eq' t1 t2 -> sub_trace t1 t2.
+  Proof. unfold trace_eq'; intuition. Qed.
+  Theorem trace_eq'_weakenr t1 t2 : trace_eq' t1 t2 -> sub_trace t2 t1.
+  Proof. unfold trace_eq'; intuition. Qed.
+  Theorem trace_eq_eq'_equiv t1 t2 : trace_eq t1 t2 <-> trace_eq' t1 t2.
+  Proof.
+    unfold trace_eq, trace_eq', sub_trace, set_eq;
     destruct t1; destruct t2; intuition.
-Qed.
+  Qed.
 
-Theorem trace_eq_weakenl t1 t2 : trace_eq t1 t2 -> sub_trace t1 t2.
-Proof. rewrite trace_eq_eq'_equiv; apply trace_eq'_weakenl. Qed.
+  Theorem trace_eq_weakenl t1 t2 : trace_eq t1 t2 -> sub_trace t1 t2.
+  Proof. rewrite trace_eq_eq'_equiv; apply trace_eq'_weakenl. Qed.
 
-Theorem trace_eq_weakenr t1 t2 : trace_eq t1 t2 -> sub_trace t2 t1.
-Proof. rewrite trace_eq_eq'_equiv; apply trace_eq'_weakenr. Qed.
+  Theorem trace_eq_weakenr t1 t2 : trace_eq t1 t2 -> sub_trace t2 t1.
+  Proof. rewrite trace_eq_eq'_equiv; apply trace_eq'_weakenr. Qed.
 
-Theorem trace_plus_cong t1 t2 t3 t4 : trace_eq t1 t3 -> trace_eq t2 t4 -> trace_eq (trace_plus t1 t2) (trace_plus t3 t4).
-  unfold trace_eq.
-  destruct t1; destruct t2; destruct t3; destruct t4.
-  unfold trace_plus.
-  intros H; destruct4 H.
-  intros H'; destruct4 H'.
-  split4; apply set_union_cong; auto.
-Qed.
+  Theorem trace_plus_cong t1 t2 t3 t4 : trace_eq t1 t3 -> trace_eq t2 t4 -> trace_eq (trace_plus t1 t2) (trace_plus t3 t4).
+    unfold trace_eq.
+    destruct t1; destruct t2; destruct t3; destruct t4.
+    unfold trace_plus.
+    intros H; destruct4 H.
+    intros H'; destruct4 H'.
+    split4; apply set_union_cong; auto.
+  Qed.
 
-Theorem trace_eq_refl t : trace_eq t t.
-Proof.
-  unfold trace_eq; destruct t; split4; apply set_eq_refl.
-Qed.
-
-
-Theorem trace_eq_symm t1 t2 : trace_eq t1 t2 -> trace_eq t2 t1.
-Proof.
-  unfold trace_eq.
-  destruct t1; destruct t2.
-  intros H; destruct4 H.
-  split4; apply set_eq_symm; auto.
-Qed.
-
-Theorem trace_eq_trans t1 t2 t3 : trace_eq t1 t2 -> trace_eq t2 t3 -> trace_eq t1 t3.
-Proof.
-  unfold trace_eq.
-  destruct t1; destruct t2; destruct t3.
-  intros H; destruct4 H.
-  intros H'; destruct4 H'.
-  split4; eapply set_eq_trans; eauto.
-Qed.
-
-Theorem trace_plus_comm t1 t2 : trace_eq (trace_plus t1 t2) (trace_plus t2 t1).
-Proof.
-  destruct t1, t2.
-  unfold trace_plus.
-  split4; apply set_eq_union_comm.
-Qed.
-
-Theorem trace_plus_assoc t1 t2 t3 : trace_eq (trace_plus t1 (trace_plus t2 t3))
-                                             (trace_plus (trace_plus t1 t2) t3).
-Proof.
-  destruct t1, t2, t3.
-  unfold trace_plus.
-  split4; apply set_eq_symm; apply set_union_assoc.
-Qed.
-
-Theorem sub_trace_plus_transl t tl tr
-: sub_trace t tl -> sub_trace t (trace_plus tl tr).
-Proof.
-  intros H; destruct t; destruct tl; destruct tr;
-  destruct4 H; split4; apply subset_union_transl; auto.
-Qed.
-
-Theorem sub_trace_plus_transr t tl tr
-: sub_trace t tr -> sub_trace t (trace_plus tl tr).
-Proof.
-  intros H.
-  eapply sub_trace_trans.
-  Focus 2.
-  apply trace_eq_weakenl.
-  apply trace_plus_comm.
-  apply sub_trace_plus_transl; auto.
-Qed.
-
-Theorem trace_lt_from_to_0_same e n : trace_eq (Trace_lt e n) (Trace_from_to e 0 n).
-Proof.
-  induction n.
-  simpl.
-  split4; apply set_eq_refl.
-
-  simpl.
-  unfold trace_plus.
-  destruct (Trace_on e n).
-  destruct (Trace_lt e n).
-  destruct (Trace_from_to e 0 n).
-  destruct4 IHn.
-  split4; (apply set_union_cong; [apply set_eq_refl|]; auto).
-Qed.
-
-Theorem trace_plus_unitl t :
-  trace_eq (trace_plus trace_zero t) t.
-Proof.
-  destruct t; split4; apply set_union_unitl.
-Qed.
-
-Theorem trace_plus_unitl_gen t1 t2 :
-  trace_eq t1 t2 -> trace_eq (trace_plus trace_zero t1) t2.
-Proof.
-  intros H.
-  eapply trace_eq_trans; [ apply trace_plus_unitl | auto].
-Qed.
+  Theorem trace_eq_refl t : trace_eq t t.
+  Proof.
+    unfold trace_eq; destruct t; split4; apply set_eq_refl.
+  Qed.
 
 
-Theorem trace_plus_unitr t :
-  trace_eq (trace_plus t trace_zero) t.
-Proof.
-  eapply trace_eq_trans;
-  [apply trace_plus_comm| apply trace_plus_unitl].
-Qed.
+  Theorem trace_eq_symm t1 t2 : trace_eq t1 t2 -> trace_eq t2 t1.
+  Proof.
+    unfold trace_eq.
+    destruct t1; destruct t2.
+    intros H; destruct4 H.
+    split4; apply set_eq_symm; auto.
+  Qed.
+
+  Theorem trace_eq_trans t1 t2 t3 : trace_eq t1 t2 -> trace_eq t2 t3 -> trace_eq t1 t3.
+  Proof.
+    unfold trace_eq.
+    destruct t1; destruct t2; destruct t3.
+    intros H; destruct4 H.
+    intros H'; destruct4 H'.
+    split4; eapply set_eq_trans; eauto.
+  Qed.
+
+  Theorem trace_plus_comm t1 t2 : trace_eq (trace_plus t1 t2) (trace_plus t2 t1).
+  Proof.
+    destruct t1, t2.
+    unfold trace_plus.
+    split4; apply set_eq_union_comm.
+  Qed.
+
+  Theorem trace_plus_assoc t1 t2 t3 : trace_eq (trace_plus t1 (trace_plus t2 t3))
+                                               (trace_plus (trace_plus t1 t2) t3).
+  Proof.
+    destruct t1, t2, t3.
+    unfold trace_plus.
+    split4; apply set_eq_symm; apply set_union_assoc.
+  Qed.
+
+  Theorem sub_trace_plus_transl t tl tr
+  : sub_trace t tl -> sub_trace t (trace_plus tl tr).
+  Proof.
+    intros H; destruct t; destruct tl; destruct tr;
+    destruct4 H; split4; apply subset_union_transl; auto.
+  Qed.
+
+  Theorem sub_trace_plus_transr t tl tr
+  : sub_trace t tr -> sub_trace t (trace_plus tl tr).
+  Proof.
+    intros H.
+    eapply sub_trace_trans.
+    Focus 2.
+    apply trace_eq_weakenl.
+    apply trace_plus_comm.
+    apply sub_trace_plus_transl; auto.
+  Qed.
+
+  Theorem trace_plus_unitl t :
+    trace_eq (trace_plus trace_zero t) t.
+  Proof.
+    destruct t; split4; apply set_union_unitl.
+  Qed.
+
+  Theorem trace_plus_unitl_gen t1 t2 :
+    trace_eq t1 t2 -> trace_eq (trace_plus trace_zero t1) t2.
+  Proof.
+    intros H.
+    eapply trace_eq_trans; [ apply trace_plus_unitl | auto].
+  Qed.
 
 
-Theorem trace_plus_unitr_gen t1 t2 :
-  trace_eq t1 t2 -> trace_eq (trace_plus t1 trace_zero) t2.
-Proof.
-  intros H.
-  eapply trace_eq_trans; [ apply trace_plus_unitr | auto].
-Qed.
-
-Theorem trace_from_to_ge e m n
-: n <= m ->
-  Trace_from_to e m n = trace_zero.
-Proof.
-  intros H.
-  unfold Trace_from_to.
-  remember (le_lt_dec n m) as l.
-  destruct l; [| apply False_ind; nliamega ].
-  destruct n; rewrite <-Heql; reflexivity.
-Qed.
-
-Theorem trace_from_to_self e m 
-: Trace_from_to e m m = trace_zero.
-Proof. apply trace_from_to_ge; nliamega. Qed.
-
-Theorem trace_from_to_split1r e m n
-: m <= n ->
-  trace_eq (Trace_from_to e m (S n))
-           (trace_plus (Trace_from_to e m n) (Trace_on e n)).
-Proof.
-  intros H.
-  unfold Trace_from_to at 1.
-  remember (le_lt_dec (S n) m).
-  destruct s.
-  assert (S n <= n).
-  apply le_trans with (m := m); auto.
-  apply le_Sn_n in H0.
-  contradiction.
-  fold Trace_from_to.
-  apply trace_plus_comm.
-Qed.
-
-Theorem trace_from_to_split1l' e m n
-: trace_eq (Trace_from_to e m (S (m + n)))
-           (trace_plus (Trace_on e m) (Trace_from_to e (S m) (S (m + n)))).
-Proof.
-  generalize dependent m.
-  induction n as [| n].
-  intros m.
-  replace (S (m + 0)) with (S m) by nliamega.
-  unfold Trace_from_to at 1.
-  remember (le_lt_dec (S m) m) as t.
-  destruct t.
-  clear Heqt.
-  apply le_Sn_n in l.
-  contradiction.
-
-  fold Trace_from_to.
-  rewrite trace_from_to_self.
-  rewrite trace_from_to_self.
-  apply trace_eq_refl.
-  intros m.
-  unfold Trace_from_to.
-  remember (le_lt_dec (S (m + S n)) m) as t.
-  destruct t.
-  assert (m < (S (m + S n))) by nliamega.
-  clear Heqt.
-  apply (le_not_gt) in l.
-  contradiction.
-  fold Trace_from_to.
-  clear l Heqt.
-  remember (le_lt_dec (S (m + S n)) (S m)).
-  destruct s.
-  assert ((S (m + S n)) > S m) by nliamega.
-  clear Heqs; apply le_not_gt in l; contradiction.
-  replace (m + S n) with (S (m + n)) by nliamega.
-  eapply trace_eq_trans.
-  apply trace_plus_cong; [apply trace_eq_refl | apply IHn ].
-  eapply trace_eq_trans.
-  apply trace_plus_assoc.
-  eapply trace_eq_trans.
-  apply trace_plus_cong.
-  apply trace_plus_comm.
-  apply trace_eq_refl.
-  eapply trace_eq_trans.
-  apply trace_eq_symm.
-  apply trace_plus_assoc.
-  apply trace_eq_refl.
-Qed.
-
-Theorem trace_from_to_split1l e m n
-: m < n ->
-  trace_eq (Trace_from_to e m n)
-           (trace_plus (Trace_on e m) (Trace_from_to e (S m) n)).
-Proof.
-  intros H.
-  remember (pred (n - m)) as t.
-  assert (n = (S (m + t))) by nliamega.
-  subst n.
-  apply trace_from_to_split1l'.
-Qed.
+  Theorem trace_plus_unitr t :
+    trace_eq (trace_plus t trace_zero) t.
+  Proof.
+    eapply trace_eq_trans;
+    [apply trace_plus_comm| apply trace_plus_unitl].
+  Qed.
 
 
-Theorem trace_from_to_split e m n p :
-  (m <= n < p)
-  -> trace_eq (Trace_from_to e m p)
-              (trace_plus (Trace_from_to e m n)
-                          (Trace_from_to e n p)).
-Proof.
-  generalize dependent p.
-  generalize dependent m.
+  Theorem trace_plus_unitr_gen t1 t2 :
+    trace_eq t1 t2 -> trace_eq (trace_plus t1 trace_zero) t2.
+  Proof.
+    intros H.
+    eapply trace_eq_trans; [ apply trace_plus_unitr | auto].
+  Qed.
 
-  induction n.
-  intros m p [Hmzero Hppos].
-  apply le_n_0_eq in Hmzero; subst.
-  remember (Trace_from_to e 0 0).
-  simpl in Heqt; subst.
-  apply trace_eq_symm.
-  apply trace_plus_unitl.
+End Traces.
+Hint Resolve trace_eq_refl.
+Hint Resolve sub_trace_refl.
 
-  intros m p [Hmn Hp].
-  inversion Hmn; subst.
-  clear Hmn.
-  apply trace_eq_symm.
-  rewrite (trace_from_to_self e (S n)).
-  apply trace_plus_unitl_gen.
-  apply trace_eq_refl.
+Section Enumerates.
+  Inductive Enumerates : Enum -> nat -> Value -> Trace -> Prop :=
+  | ES_Nat :
+      forall n,
+        Enumerates E_Nat n (V_Nat n) trace_zero
+  | ES_Pair :
+      forall l r n ln rn lx rx lt rt,
+        Pairing n ln rn ->
+        Enumerates l ln lx lt ->
+        Enumerates r rn rx rt ->
+        Enumerates (E_Pair l r) n (V_Pair lx rx) (trace_plus lt rt)
+  | ES_Map :
+      forall bi inner inner_x n x t,
+        Bijects bi x inner_x ->
+        Enumerates inner n inner_x t ->
+        Enumerates (E_Map bi inner) n x t
+  | ES_Dep:
+      forall l f n ln rn lx rx lt rt,
+        Pairing n ln rn ->
+        Enumerates l ln lx lt ->
+        Enumerates (f lx) rn rx rt ->
+        Enumerates (E_Dep l f) n (V_Pair lx rx) (trace_plus lt rt)
+  | ES_Sum_Left:
+      forall l r n ln lx t,
+        n = 2 * ln ->
+        Enumerates l ln lx t ->
+        Enumerates (E_Sum l r) n (V_Sum_Left lx) t
+  | ES_Sum_Right:
+      forall l r n rn rx t,
+        n = 2 * rn + 1 ->
+        Enumerates r rn rx t ->
+        Enumerates (E_Sum l r) n (V_Sum_Right rx) t
+  (* E_Trace hides traces below it. This makes traces super easily spoofable, but makes it easier to reason about when they're not spoofed *)
+  | ES_Trace :
+      forall n tg e v _t,
+        Enumerates e n v _t ->
+        Enumerates (E_Trace tg e) n v (trace_one n tg).
+  Hint Constructors Enumerates.
 
-  apply trace_eq_trans with (t2:= (trace_plus (Trace_from_to e m n) (Trace_from_to e n p)));
-    [apply IHn; nliamega| ].
-  apply trace_eq_trans with (t2 := (trace_plus (Trace_from_to e m n)
-                                               (trace_plus (Trace_on e n)
-                                                           (Trace_from_to e (S n) p)))).
-  apply trace_plus_cong; [apply trace_eq_refl| ].
-  apply trace_from_to_split1l; nliamega.
+  (* Couldn't prove this with traces assumed to be equal. *)
+  Theorem Enumerates_to_fun :
+    forall e x n1 n2 t1 t2,
+      Enumerates e n1 x t1 ->
+      Enumerates e n2 x t2 ->
+      n1 = n2.
+  Proof.
+    induction e; intros x n1 n2 t1 t2 E1 E2; inversion E1; inversion E2; subst; try congruence.
 
-  eapply trace_eq_trans.
-  apply trace_plus_assoc.
-  apply trace_plus_cong; [| apply trace_eq_refl].
-  apply trace_eq_symm.
-  apply trace_from_to_split1r; nliamega.
-Qed.
+    (* E_Pair *)
+    - replace lx0 with lx in *; try congruence.
+      replace rx0 with rx in *; try congruence.
+      erewrite (IHe1 _ _ _ _ _ H2 H10) in *.
+      erewrite (IHe2 _ _ _ _ _ H6 H14) in *.
+      erewrite (Pairing_from_fun _ _ _ _ H1 H9) in *.
+      auto.
 
-Theorem trace_from_to_0_split :
-  forall m n e,
-    m < n ->
-    trace_eq (Trace_lt e n)
-             (trace_plus (Trace_lt e m)
-                         (Trace_from_to e m n)).
-Proof.
-  intros m n e Hmn.
-  eapply trace_eq_trans.
-  apply trace_lt_from_to_0_same.
-  eapply trace_eq_trans.
-  apply trace_from_to_split with (n := m); split; [nliamega | assumption].
-  apply trace_plus_cong.
-  apply trace_eq_symm.
-  apply trace_lt_from_to_0_same.
-  apply trace_eq_refl.
-Qed.
+    (* E_Map *)
+    - erewrite (Bijects_fun_right _ _ _ _ _ _ H1 H8) in *.
+      erewrite (IHe _ _ _ _ _ H5 H12) in *.
+      auto.
 
+    (* E_Dep *)
+    - inversion H13.
+      subst.
+      erewrite (IHe _ _ _ _ _ H3 H11) in *.
+      erewrite (H _ _ _ _ _ _ H7 H15) in *.
+      erewrite (Pairing_from_fun _ _ _ _ H2 H10) in *.
+      auto.
 
-Theorem Trace_nat n tg : Trace_on (E_Trace tg E_Nat) n = trace_one n tg.
-Proof.
-  unfold Trace_on.
-  destruct (Enumerates_from_dec _ _) as [[v t] Henum].
-  inversion Henum; subst.
-  reflexivity.
-Qed.
+    (* E_Sum Left *)
+    - inversion H10; subst.
+      erewrite (IHe1 _ _ _ _ _ H5 H12).
+      auto.
 
-Theorem trace_off tg1 tg2 n : tg1 <> tg2 -> trace_proj tg2 (Trace_on (E_Trace tg1 E_Nat) n) = empty_set'.
-Proof.
-  rewrite Trace_nat.
-  compute.
-  destruct tg1; destruct tg2; intuition.
-Qed.
+    (* E_Sum Right *)
+    - inversion H10; subst.
+      erewrite (IHe2 _ _ _ _ _ H5 H12).
+      auto.
 
-Theorem trace_proj_plus_distrl tg t1 t2
-: trace_proj tg (trace_plus t1 t2) = (set_union' (trace_proj tg t1) (trace_proj tg t2)).
-Proof.
-  destruct t1; destruct t2; destruct tg; auto.
-Qed.
+    (* E_Trace *)
+    - apply IHe with (x := x) (t1 := _t) (t2 := _t0); assumption.
+  Qed.
 
-Theorem Trace_on_correct e n x t : Enumerates e n x t -> Trace_on e n = t.
-Proof.
-  intros H.
-  unfold Trace_on.
-  destruct (Enumerates_from_dec e n) as [[v tgaf] Henum].
-  simpl.
-  destruct (Enumerates_from_fun _ _ _ _ _ _ H Henum); auto.
-Qed.
+  Lemma even_fun:
+    forall x y,
+      2 * x = 2 * y ->
+      x = y.
+  Proof.
+    induction x as [|x]; intros; nliamega.
+  Qed.
 
-Theorem trace_lt_Nat n tg
-: set_eq (z_to_n n)
-     (trace_proj tg (Trace_lt (E_Trace tg E_Nat) n)).
-Proof.
-  induction n as [| n IHn]; [destruct tg; compute; tauto|].
-  unfold Trace_lt. fold Trace_lt.
-  unfold z_to_n. fold z_to_n.
-  rewrite trace_proj_plus_distrl.
-  rewrite Trace_nat.
-  eapply set_eq_trans.
-  apply set_eq_symm. apply set_add_cons_eq.
-  eapply set_eq_trans.
-  replace (n :: z_to_n n) with ((n :: nil) ++ z_to_n n) by reflexivity.
-  apply set_eq_symm; apply set_union_app_eq.
-  apply set_union_cong; auto.
-  destruct tg; compute; tauto.
-Qed.
+  Lemma odd_neq_even:
+    forall x y,
+      2 * x = 2 * y + 1 ->
+      False.
+  Proof.
+    induction x as [|x]; intros; nliamega.
+  Qed.
 
-Theorem trace_lt_Nat_off n tg1 tg2
-: tg1 <> tg2 ->
-  (trace_proj tg1 (Trace_lt (E_Trace tg2 E_Nat) n)) = nil.
-Proof.
-  intros Hdiff.
-  induction n.
-  destruct tg1; auto.
-  unfold Trace_lt; fold Trace_lt.
-  rewrite trace_proj_plus_distrl.
-  rewrite trace_off.
-  rewrite IHn; compute; auto.
-  auto.
-Qed.
+  Lemma odd_fun:
+    forall x y,
+      2 * x + 1 = 2 * y + 1 ->
+      x = y.
+  Proof.
+    induction x as [|x]; intros; nliamega.
+  Qed.
 
-Lemma sub_trace_from_tol l m n e
-: l <= m
-  -> sub_trace (Trace_from_to e m n) (Trace_from_to e l n).
-Proof.
-  intros H; remember (m - l) as k; replace m with (l + k) by nliamega; clear dependent m.
-  induction k.
-  replace (l + 0) with l by nliamega; apply sub_trace_refl.
-  eapply sub_trace_trans; [| apply IHk].
-  destruct (le_dec n (l + S k)).
-  rewrite trace_from_to_ge by assumption;
-    apply sub_trace_zero.
-  eapply sub_trace_trans;
-    [| apply trace_eq_weakenl; apply trace_eq_symm; apply trace_from_to_split with (n := l + S k); nliamega ];
-    apply sub_trace_plus_transr; apply sub_trace_refl.
-Qed.
+  Theorem Enumerates_from_fun :
+    forall e n x1 x2 t1 t2,
+      Enumerates e n x1 t1 ->
+      Enumerates e n x2 t2 ->
+      x1 = x2 /\ t1 = t2.
+  Proof.
+    induction e; intros x n1 n2 t1 t2 E1 E2; inversion E1; inversion E2; eauto; subst; try congruence.
 
-Theorem sub_trace_from_to l m n p e
-: l <= m
-  -> n <= p
-  -> sub_trace (Trace_from_to e m n) (Trace_from_to e l p).
-Proof.
-  intros Hlm Hnp.
-  remember (p - n) as k; replace p with (n + k) by nliamega; clear dependent p.
-  induction k.
-  replace (n+0) with n by nliamega; apply sub_trace_from_tol; auto.
-  replace (n + S k) with (S (n + k)) by nliamega.
-  unfold Trace_from_to at 2.
-  remember (le_lt_dec (S (n + k)) l) as Hlelt.
-  destruct Hlelt.
-  replace (Trace_from_to e l (n + k)) with trace_zero in IHk; auto.
-  symmetry.
-  apply trace_from_to_ge; nliamega.
-  fold Trace_from_to.
-  apply sub_trace_plus_transr; auto.
-Qed.
+    (* E_Pair *)
+    - erewrite (Pairing_to_l_fun _ _ _ _ _ H1 H9) in *.
+      erewrite (Pairing_to_r_fun _ _ _ _ _ H1 H9) in *.
+      destruct (IHe1 _ _ _ _ _ H2 H10); subst.
+      destruct (IHe2 _ _ _ _ _ H6 H14); subst.
+      auto.
 
-Theorem trace_from_to_Nat_off m n tg1 tg2
-: tg1 <> tg2 ->
-  (trace_proj tg1 (Trace_from_to (E_Trace tg2 E_Nat) m n)) = empty_set'.
-Proof.
-  intros Hdiff.
-  assert (sub_trace (Trace_from_to (E_Trace tg2 E_Nat) m n) (Trace_lt (E_Trace tg2 E_Nat) n)).
-  eapply sub_trace_trans.
-  apply sub_trace_from_to with (l := 0) (p := n); try nliamega.
-  apply trace_eq_weakenl; apply trace_eq_symm; apply trace_lt_from_to_0_same.
-  apply subset_nil_nil.
-  erewrite <-trace_lt_Nat_off; [ apply sub_trace_proj|]; eauto.
-Qed.
+    (* E_Map *)
+    - destruct (IHe _ _ _ _ _ H5 H12); subst.
+      erewrite (Bijects_fun_left _ _ _ _ _ _ H1 H8) in *.
+      auto.
 
-Theorem trace_on_Pair_off tg e1 e2 m
-: (forall n, trace_proj tg (Trace_on e1 n) = empty_set')
-  -> (forall n, trace_proj tg (Trace_on e2 n) = empty_set')
-  -> trace_proj tg (Trace_on (E_Pair e1 e2) m) = empty_set'.
-Proof.
-  intros.
-  unfold Trace_on.
-  destruct (Enumerates_from_dec _ _) as [[v t] Henum].
-  inversion Henum; subst.
-  apply Trace_on_correct in H4.
-  apply Trace_on_correct in H8.
-  simpl.
-  subst.
-  rewrite trace_proj_plus_distrl.
-  rewrite H, H0.
-  trivial.
-Qed.
+    (* E_Dep *)
+    - erewrite (Pairing_to_l_fun _ _ _ _ _ H2 H10) in *.
+      erewrite (Pairing_to_r_fun _ _ _ _ _ H2 H10) in *.
+      destruct (IHe _ _ _ _ _ H3 H11); subst.
+      destruct (H _ _ _ _ _ _ H7 H15); subst.
+      auto.
 
-Theorem trace_lt_Pair_off tg e1 e2 m
-: (forall n, trace_proj tg (Trace_on e1 n) = empty_set')
-  -> (forall n, trace_proj tg (Trace_on e2 n) = empty_set')
-  -> trace_proj tg (Trace_lt (E_Pair e1 e2) m) = empty_set'.
-Proof.
-  induction m; [intros; destruct tg; reflexivity|].
-  intros H1 H2.
-  unfold Trace_lt; fold Trace_lt.
-  rewrite trace_proj_plus_distrl.
-  apply subset_nil_nil.
-  apply subset_union_both.
-  rewrite trace_on_Pair_off; [apply subset_refl| |]; auto.
-  rewrite IHm; auto.
-Qed.
+    (* E_Sum Left *)
+    - erewrite (even_fun _ _ H8) in *.
+      destruct (IHe1 _ _ _ _ _ H5 H12); subst.
+      auto.
 
-Eval compute in (Trace_lt (E_Sum (E_Trace zero E_Nat) (E_Trace one E_Nat)) 20).
-Eval compute in (Trace_lt (E_Sum (E_Trace zero E_Nat) (E_Trace one E_Nat)) 21).
-Eval compute in (Trace_lt (E_Sum (E_Trace zero E_Nat) (E_Trace one E_Nat)) 22).
-Eval compute in (Trace_lt (E_Sum (E_Trace zero E_Nat) (E_Trace one E_Nat)) 23).
-Eval compute in (Trace_lt (E_Sum (E_Trace zero E_Nat) (E_Trace one E_Nat)) 24).
-Eval compute in (z_to_n 10).
-Eval compute in (Trace_lt (E_Sum (E_Trace zero E_Nat) (E_Trace one E_Nat)) 20).
+    (* E_Sum Left & Right *)
+    - apply odd_neq_even in H8. contradiction.
+
+    (* E_Sum Right & Left *)
+    - subst. symmetry in H8. apply odd_neq_even in H8. contradiction.
+
+    (* E_Sum Right *)
+    - erewrite (odd_fun _ _ H8) in *.
+      destruct (IHe2 _ _ _ _ _ H5 H12); subst.
+      auto.
+
+    (* E_Trace *)
+    - destruct (IHe _ _ _ _ _ H4 H10); subst.
+      auto.
+  Qed.
+
+  (* Map/Trace compatibility lemmas *)
+  Lemma Enumerates_to_dec_Map :
+    forall b e x,
+      (forall x,
+         { nt: nat * Trace | let (n, t) := nt in Enumerates e n x t }
+         + { forall n t, ~ Enumerates e n x t }) ->
+      { nt : nat * Trace | let (n, t) := nt in Enumerates (E_Map b e) n x t }
+      + { forall n t, ~ Enumerates (E_Map b e) n x t }.
+  Proof.
+    intros b e x IHe.
+    destruct (Bijects_to_dec _ _ b x) as [y B].
+    destruct (IHe y) as [[nt IHE] | NIH].
+
+    left. exists nt. destruct nt. eauto.
+
+    right. intros n t E.
+    inversion E. subst n0 x0 t0 inner bi.
+    rename H1 into B'. rename H5 into IHE.
+    erewrite (Bijects_fun_right _ _ _ _ _ _ B B') in *.
+    eapply NIH. apply IHE.
+  Defined.
+  Hint Resolve Enumerates_to_dec_Map.
+
+  Lemma Enumerates_to_dec_Trace :
+    forall tg e x,
+      (forall x,
+         { nt: nat * Trace | let (n, t) := nt in Enumerates e n x t }
+         + { forall n t, ~ Enumerates e n x t }) ->
+      { nt : nat * Trace | let (n, t) := nt in Enumerates (E_Trace tg e) n x t }
+      + { forall n t, ~ Enumerates (E_Trace tg e) n x t }.
+  Proof.
+    intros tg e x IHe.
+    destruct (IHe x) as [[[n t] IHE] | NIH].
+
+    left.
+    exists (n, trace_one n tg); eauto.
+
+    right.
+    intros n t E.
+    inversion E; eapply NIH; eauto.
+  Defined.
+  Hint Resolve Enumerates_to_dec_Trace.
 
 
-(* Proof idea: equilibrium = 2 * n + 2,  uses = 0..(S n) *)
-Theorem Sum_Fair : Fair2 E_Sum.
-Proof.
-  unfold Fair2.
-  intros n.
-  exists (2 * n + 2).
-  remember (Trace_lt (E_Sum (E_Trace zero E_Nat) (E_Trace one E_Nat)) (2 * n + 2)).
-  destruct t as [tz to ttw tth].
-  split; [nliamega| ].
+  Definition Enumerates_to_dec:
+    forall e x,
+      { nt : nat * Trace | let (n, t) := nt in Enumerates e n x t } + { forall n t, ~ Enumerates e n x t }.
+  Proof.
+    induction e; destruct x; eauto;
+    try ( right; intros _n _t E; inversion E; fail ).
 
-  generalize dependent tth.
-  generalize dependent ttw.
-  generalize dependent to.
-  generalize dependent tz.
-  induction n.
-  intros tz to ttw tth Heqt.
-  inversion Heqt; auto; apply set_eq_refl.
+    (* E_Nat *)
+    - left; exists (n, trace_zero); constructor.
 
-  intros tz to ttw tth Htzto.
-  remember (Trace_lt (E_Sum (E_Trace zero E_Nat) (E_Trace one E_Nat)) (2 * n + 2)).
-  replace (2 * S n + 2) with (S (S (2 * n + 2))) in Htzto by nliamega.
-  simpl in Htzto.
-  replace (n + (n + 0) + 2) with (2 * n + 2) in Htzto by nliamega.
-  destruct t as [tz' to' ttw' tth'].
-  assert (set_eq tz' to').
-  eapply IHn ; auto.
-  rewrite <-Heqt in Htzto.
-  clear Heqt.
-  clear IHn.
-  replace (Trace_on (E_Sum (E_Trace zero E_Nat) (E_Trace one E_Nat)) (S (2 * n + 2))) with (trace_one (S n) one) in Htzto.
+    (* E_Pair *)
+    - rename x1 into lx. rename x2 into rx.
+      rename e1 into l. rename e2 into r.
+      destruct (IHe1 lx) as [[[ln lt] EL] | LF].
+      destruct (IHe2 rx) as [[[rn rt] ER] | RF].
+      left.
+      destruct (Pairing_to_dec ln rn) as [n P].
+      exists (n, trace_plus lt rt).
+      eauto.
 
-  replace (Trace_on (E_Sum (E_Trace zero E_Nat) (E_Trace one E_Nat)) ((2 * n)+2)) with (trace_one (S n) zero) in Htzto.
-  unfold trace_one in Htzto.
-  unfold trace_plus in Htzto.
-  inversion Htzto.
-  clear  Htzto H1 H2.
+      right. intros _n _t E; inversion E; subst.
+      eapply RF; eauto.
 
-  - SearchAbout set_eq.
-    apply set_eq_trans with (s2 := set_union' (S n :: nil) tz').
-    apply set_union_unitl.
-    apply set_eq_trans with (s2 := set_union' (S n :: nil) to').
+      right. intros _n _t E; inversion E; subst.
+      eapply LF; eauto.
+
+    (* E_Dep *)
+    - destruct (IHe x1) as [[[ln lt] EL] | LF].
+      destruct (X x1 x2) as [[[rn rt] ER] | RF].
+      left.
+      destruct (Pairing_to_dec ln rn) as [n P].
+      exists (n, trace_plus lt rt).
+      eauto.
+
+      right. intros _n _t E; inversion E; subst.
+      eapply RF; eauto.
+
+      right. intros _n _t E; inversion E; subst.
+      eapply LF; eauto.
+
+    (* E_Sum Left *)
+    - destruct (IHe1 x) as [[[ln lt] EL] | LF].
+      left. exists (2 * ln, lt). eauto.
+
+      right. intros _n _t E. inversion E; subst.
+      eapply LF; eauto.
+
+    (* E_Sum Right *)
+    - destruct (IHe2 x) as [[[rn rt] ER] | RF].
+      left. exists (2 * rn + 1, rt). eauto.
+
+      right. intros _n _t E. inversion E; subst.
+      eapply RF; eauto.
+  Defined.
+
+  Lemma even_SS :
+    forall n,
+      { l | n = 2 * l } -> { m | S (S n) = 2 * m }.
+  Proof.
+    intros n P.
+    destruct P.
+    exists ((S x)).
+    nliamega.
+  Defined.
+
+  Lemma odd_SS :
+    forall n,
+      { r | n = 2 * r + 1 } -> { m | S (S n) = 2 * m + 1 }.
+  Proof.
+    intros n P.
+    destruct P.
+    exists ((S x)).
+    nliamega.
+  Defined.
+
+  Fixpoint even_odd_eq_dec n : { l | n = 2 * l } + { r | n = 2 * r + 1 }.
+  Proof.
+    refine (match n with
+              | 0 => _
+              | S 0 => _
+              | S (S n') => _
+            end).
+    left;  exists 0; auto.
+    right; exists 0; auto.
+
+    clear n0.
+    destruct (even_odd_eq_dec n').
+    left; apply even_SS; assumption.
+    right; apply odd_SS; assumption.
+  Defined.
+
+  Definition Enumerates_from_dec:
+    forall e n,
+      { xt : Value * Trace | let (x, t) := xt in Enumerates e n x t }.
+  Proof.
+    induction e; intros n; eauto.
+
+    (* E_Nat *)
+    - exists (V_Nat n, trace_zero); eauto.
+
+    (* E_pair *)
+    - rename e1 into l. rename e2 into r.
+      remember (Pairing_from n) as PF.
+      destruct PF as [ln rn].
+      destruct (IHe1 ln) as [[lx lt] EL].
+      destruct (IHe2 rn) as [[rx rt] ER].
+      exists (V_Pair lx rx, trace_plus lt rt).
+      eauto.
+
+    (* E_Map *)
+    - destruct (IHe n) as [[x t] IHE].
+      destruct (Bijects_from_dec _ _ b x) as [y B].
+      exists (y, t). eauto.
+
+    (* E_Dep *)
+    - rename e into l. rename e0 into f.
+      remember (Pairing_from n) as PF.
+      destruct PF as [ln rn].
+      destruct (IHe ln) as [[lx lt] EL].
+      destruct (X lx rn) as [[rx rt] ER].
+      exists (V_Pair lx rx, trace_plus lt rt). eauto.
+
+    (* E_Sum *)
+    - destruct (even_odd_dec n) as [Hev | Hodd].
+      apply even_double in Hev.
+      destruct (IHe1 (div2 n)) as [[lx lt] EL].
+      exists (V_Sum_Left lx, lt).
+      rewrite double_twice in Hev.
+      eauto.
+
+      apply odd_double in Hodd.
+      destruct (IHe2 (div2 n)) as [[rx rt] ER].
+      exists (V_Sum_Right rx, rt).
+      rewrite double_twice in Hodd.
+      replace (S (2 * div2 n)) with (2 * div2 n + 1) in Hodd by nliamega.
+      eauto.
+
+    (* E_Trace *)
+    - rename t into tg.
+      destruct (IHe n) as [[x _t] E].
+      exists (x, trace_one n tg).
+      eauto.
+  Defined.
+End Enumerates.
+Hint Constructors Enumerates.
+Hint Resolve Enumerates_to_dec_Trace.
+Hint Resolve Enumerates_to_dec_Map.
+
+
+Section EnumTrace.
+  Definition Trace_on (e : Enum) (n : nat) : Trace :=
+    let (nt, _) := (Enumerates_from_dec e n) in snd nt.
+
+  Fixpoint Trace_lt (e : Enum) n : Trace :=
+    match n with
+      | 0 => trace_zero
+      | S n' => trace_plus (Trace_on e n') (Trace_lt e n')
+    end.
+
+  Fixpoint Trace_from_to e lo hi : Trace :=
+    if le_lt_dec hi lo
+    then trace_zero
+    else match hi with
+           | 0 => trace_zero
+           | S hi' => trace_plus (Trace_on e hi') (Trace_from_to e lo hi')
+         end.
+
+  Theorem trace_lt_from_to_0_same e n : trace_eq (Trace_lt e n) (Trace_from_to e 0 n).
+  Proof.
+    induction n.
+    simpl.
+    split4; apply set_eq_refl.
+
+    simpl.
+    unfold trace_plus.
+    destruct (Trace_on e n).
+    destruct (Trace_lt e n).
+    destruct (Trace_from_to e 0 n).
+    destruct4 IHn.
+    split4; (apply set_union_cong; [apply set_eq_refl|]; auto).
+  Qed.
+
+  Theorem trace_from_to_ge e m n
+  : n <= m ->
+    Trace_from_to e m n = trace_zero.
+  Proof.
+    intros H.
+    unfold Trace_from_to.
+    remember (le_lt_dec n m) as l.
+    destruct l; [| apply False_ind; nliamega ].
+    destruct n; rewrite <-Heql; reflexivity.
+  Qed.
+
+  Theorem trace_from_to_self e m 
+  : Trace_from_to e m m = trace_zero.
+  Proof. apply trace_from_to_ge; nliamega. Qed.
+
+  Theorem trace_from_to_split1r e m n
+  : m <= n ->
+    trace_eq (Trace_from_to e m (S n))
+             (trace_plus (Trace_from_to e m n) (Trace_on e n)).
+  Proof.
+    intros H.
+    unfold Trace_from_to at 1.
+    remember (le_lt_dec (S n) m).
+    destruct s.
+    assert (S n <= n).
+    apply le_trans with (m := m); auto.
+    apply le_Sn_n in H0.
+    contradiction.
+    fold Trace_from_to.
+    apply trace_plus_comm.
+  Qed.
+
+  Theorem trace_from_to_split1l' e m n
+  : trace_eq (Trace_from_to e m (S (m + n)))
+             (trace_plus (Trace_on e m) (Trace_from_to e (S m) (S (m + n)))).
+  Proof.
+    generalize dependent m.
+    induction n as [| n].
+    intros m.
+    replace (S (m + 0)) with (S m) by nliamega.
+    unfold Trace_from_to at 1.
+    remember (le_lt_dec (S m) m) as t.
+    destruct t.
+    clear Heqt.
+    apply le_Sn_n in l.
+    contradiction.
+
+    fold Trace_from_to.
+    rewrite trace_from_to_self.
+    rewrite trace_from_to_self.
+    apply trace_eq_refl.
+    intros m.
+    unfold Trace_from_to.
+    remember (le_lt_dec (S (m + S n)) m) as t.
+    destruct t.
+    assert (m < (S (m + S n))) by nliamega.
+    clear Heqt.
+    apply (le_not_gt) in l.
+    contradiction.
+    fold Trace_from_to.
+    clear l Heqt.
+    remember (le_lt_dec (S (m + S n)) (S m)).
+    destruct s.
+    assert ((S (m + S n)) > S m) by nliamega.
+    clear Heqs; apply le_not_gt in l; contradiction.
+    replace (m + S n) with (S (m + n)) by nliamega.
+    eapply trace_eq_trans.
+    apply trace_plus_cong; [apply trace_eq_refl | apply IHn ].
+    eapply trace_eq_trans.
+    apply trace_plus_assoc.
+    eapply trace_eq_trans.
+    apply trace_plus_cong.
+    apply trace_plus_comm.
+    apply trace_eq_refl.
+    eapply trace_eq_trans.
+    apply trace_eq_symm.
+    apply trace_plus_assoc.
+    apply trace_eq_refl.
+  Qed.
+
+  Theorem trace_from_to_split1l e m n
+  : m < n ->
+    trace_eq (Trace_from_to e m n)
+             (trace_plus (Trace_on e m) (Trace_from_to e (S m) n)).
+  Proof.
+    intros H.
+    remember (pred (n - m)) as t.
+    assert (n = (S (m + t))) by nliamega.
+    subst n.
+    apply trace_from_to_split1l'.
+  Qed.
+
+
+  Theorem trace_from_to_split e m n p :
+    (m <= n < p)
+    -> trace_eq (Trace_from_to e m p)
+                (trace_plus (Trace_from_to e m n)
+                            (Trace_from_to e n p)).
+  Proof.
+    generalize dependent p.
+    generalize dependent m.
+
+    induction n.
+    intros m p [Hmzero Hppos].
+    apply le_n_0_eq in Hmzero; subst.
+    remember (Trace_from_to e 0 0).
+    simpl in Heqt; subst.
+    apply trace_eq_symm.
+    apply trace_plus_unitl.
+
+    intros m p [Hmn Hp].
+    inversion Hmn; subst.
+    clear Hmn.
+    apply trace_eq_symm.
+    rewrite (trace_from_to_self e (S n)).
+    apply trace_plus_unitl_gen.
+    apply trace_eq_refl.
+
+    apply trace_eq_trans with (t2:= (trace_plus (Trace_from_to e m n) (Trace_from_to e n p)));
+      [apply IHn; nliamega| ].
+    apply trace_eq_trans with (t2 := (trace_plus (Trace_from_to e m n)
+                                                 (trace_plus (Trace_on e n)
+                                                             (Trace_from_to e (S n) p)))).
+    apply trace_plus_cong; [apply trace_eq_refl| ].
+    apply trace_from_to_split1l; nliamega.
+
+    eapply trace_eq_trans.
+    apply trace_plus_assoc.
+    apply trace_plus_cong; [| apply trace_eq_refl].
+    apply trace_eq_symm.
+    apply trace_from_to_split1r; nliamega.
+  Qed.
+
+  Theorem trace_from_to_0_split :
+    forall m n e,
+      m < n ->
+      trace_eq (Trace_lt e n)
+               (trace_plus (Trace_lt e m)
+                           (Trace_from_to e m n)).
+  Proof.
+    intros m n e Hmn.
+    eapply trace_eq_trans.
+    apply trace_lt_from_to_0_same.
+    eapply trace_eq_trans.
+    apply trace_from_to_split with (n := m); split; [nliamega | assumption].
+    apply trace_plus_cong.
+    apply trace_eq_symm.
+    apply trace_lt_from_to_0_same.
+    apply trace_eq_refl.
+  Qed.
+
+  Theorem Trace_nat n tg : Trace_on (E_Trace tg E_Nat) n = trace_one n tg.
+  Proof.
+    unfold Trace_on.
+    destruct (Enumerates_from_dec _ _) as [[v t] Henum].
+    inversion Henum; subst.
+    reflexivity.
+  Qed.
+
+  Theorem trace_off tg1 tg2 n : tg1 <> tg2 -> trace_proj tg2 (Trace_on (E_Trace tg1 E_Nat) n) = empty_set'.
+  Proof.
+    rewrite Trace_nat.
+    compute.
+    destruct tg1; destruct tg2; intuition.
+  Qed.
+
+  Theorem trace_proj_plus_distrl tg t1 t2
+  : trace_proj tg (trace_plus t1 t2) = (set_union' (trace_proj tg t1) (trace_proj tg t2)).
+  Proof.
+    destruct t1; destruct t2; destruct tg; auto.
+  Qed.
+
+  Theorem Trace_on_correct e n x t : Enumerates e n x t -> Trace_on e n = t.
+  Proof.
+    intros H.
+    unfold Trace_on.
+    destruct (Enumerates_from_dec e n) as [[v tgaf] Henum].
+    simpl.
+    destruct (Enumerates_from_fun _ _ _ _ _ _ H Henum); auto.
+  Qed.
+
+  Theorem trace_lt_Nat n tg
+  : set_eq (z_to_n n)
+           (trace_proj tg (Trace_lt (E_Trace tg E_Nat) n)).
+  Proof.
+    induction n as [| n IHn]; [destruct tg; compute; tauto|].
+    unfold Trace_lt. fold Trace_lt.
+    unfold z_to_n. fold z_to_n.
+    rewrite trace_proj_plus_distrl.
+    rewrite Trace_nat.
+    eapply set_eq_trans.
+    apply set_eq_symm. apply set_add_cons_eq.
+    eapply set_eq_trans.
+    replace (n :: z_to_n n) with ((n :: nil) ++ z_to_n n) by reflexivity.
+    apply set_eq_symm; apply set_union_app_eq.
     apply set_union_cong; auto.
-    apply set_union_cong.
-    apply set_eq_refl.
-    apply set_eq_symm.
-    apply set_union_unitl.
+    destruct tg; compute; tauto.
+  Qed.
 
-  (* Trace (left + right) (2n+3) =  *)
-  - unfold Trace_on.
-    destruct (Enumerates_from_dec (E_Sum (E_Trace zero E_Nat) (E_Trace one E_Nat)) (2 * n + 2)).
-    assert (Enumerates (E_Sum (E_Trace zero E_Nat) (E_Trace one E_Nat)) (2 * n + 2) (V_Sum_Left (V_Nat (S n))) (trace_one (S n) zero)).
-    apply ES_Sum_Left with (ln := (S n)); [nliamega| ].
-    econstructor.
-    constructor.
-    destruct x.
-
-    destruct (Enumerates_from_fun _ _ _ _ _ _ y H0); subst.
+  Theorem trace_lt_Nat_off n tg1 tg2
+  : tg1 <> tg2 ->
+    (trace_proj tg1 (Trace_lt (E_Trace tg2 E_Nat) n)) = nil.
+  Proof.
+    intros Hdiff.
+    induction n.
+    destruct tg1; auto.
+    unfold Trace_lt; fold Trace_lt.
+    rewrite trace_proj_plus_distrl.
+    rewrite trace_off.
+    rewrite IHn; compute; auto.
     auto.
+  Qed.
 
-  - unfold Trace_on.
-    destruct (Enumerates_from_dec (E_Sum (E_Trace zero E_Nat) (E_Trace one E_Nat)) (S (2 * n + 2))).
-    assert (Enumerates (E_Sum (E_Trace zero E_Nat) (E_Trace one E_Nat)) (S (2 * n + 2)) (V_Sum_Right (V_Nat (S n))) (trace_one (S n) one)).
-    apply ES_Sum_Right with (rn := S n); [nliamega|].
-    econstructor; constructor.
-    destruct x.
-    destruct (Enumerates_from_fun _ _ _ _ _ _ y H0); subst.
-    auto.
-Qed.
+  Lemma sub_trace_from_tol l m n e
+  : l <= m
+    -> sub_trace (Trace_from_to e m n) (Trace_from_to e l n).
+  Proof.
+    intros H; remember (m - l) as k; replace m with (l + k) by nliamega; clear dependent m.
+    induction k.
+    replace (l + 0) with l by nliamega; apply sub_trace_refl.
+    eapply sub_trace_trans; [| apply IHk].
+    destruct (le_dec n (l + S k)).
+    rewrite trace_from_to_ge by assumption;
+      apply sub_trace_zero.
+    eapply sub_trace_trans;
+      [| apply trace_eq_weakenl; apply trace_eq_symm; apply trace_from_to_split with (n := l + S k); nliamega ];
+      apply sub_trace_plus_transr; apply sub_trace_refl.
+  Qed.
 
-Eval compute in (Trace_lt (E_Pair (E_Trace zero E_Nat) (E_Trace one E_Nat)) 0).
-Eval compute in (Trace_lt (E_Pair (E_Trace zero E_Nat) (E_Trace one E_Nat)) 1).
-Eval compute in (Trace_lt (E_Pair (E_Trace zero E_Nat) (E_Trace one E_Nat)) 4).
-Eval compute in (Trace_lt (E_Pair (E_Trace zero E_Nat) (E_Trace one E_Nat)) 9).
-Eval compute in (Trace_lt (E_Pair (E_Trace zero E_Nat) (E_Trace one E_Nat)) 16).
-Eval compute in (Trace_lt (E_Pair (E_Trace zero E_Nat) (E_Trace one E_Nat)) 25).
-Eval compute in (Trace_lt (E_Pair (E_Trace zero E_Nat) (E_Trace one E_Nat)) 36).
-Eval compute in (Trace_lt (E_Pair (E_Trace zero E_Nat) (E_Trace one E_Nat)) 49).
-Eval compute in (Trace_lt (E_Pair (E_Trace zero E_Nat) (E_Trace one E_Nat)) 64).
+  Theorem sub_trace_from_to l m n p e
+  : l <= m
+    -> n <= p
+    -> sub_trace (Trace_from_to e m n) (Trace_from_to e l p).
+  Proof.
+    intros Hlm Hnp.
+    remember (p - n) as k; replace p with (n + k) by nliamega; clear dependent p.
+    induction k.
+    replace (n+0) with n by nliamega; apply sub_trace_from_tol; auto.
+    replace (n + S k) with (S (n + k)) by nliamega.
+    unfold Trace_from_to at 2.
+    remember (le_lt_dec (S (n + k)) l) as Hlelt.
+    destruct Hlelt.
+    replace (Trace_from_to e l (n + k)) with trace_zero in IHk; auto.
+    symmetry.
+    apply trace_from_to_ge; nliamega.
+    fold Trace_from_to.
+    apply sub_trace_plus_transr; auto.
+  Qed.
 
-Definition E_PairNN := (E_Pair (E_Trace zero E_Nat) (E_Trace one E_Nat)).
+  Theorem trace_from_to_Nat_off m n tg1 tg2
+  : tg1 <> tg2 ->
+    (trace_proj tg1 (Trace_from_to (E_Trace tg2 E_Nat) m n)) = empty_set'.
+  Proof.
+    intros Hdiff.
+    assert (sub_trace (Trace_from_to (E_Trace tg2 E_Nat) m n) (Trace_lt (E_Trace tg2 E_Nat) n)).
+    eapply sub_trace_trans.
+    apply sub_trace_from_to with (l := 0) (p := n); try nliamega.
+    apply trace_eq_weakenl; apply trace_eq_symm; apply trace_lt_from_to_0_same.
+    apply subset_nil_nil.
+    erewrite <-trace_lt_Nat_off; [ apply sub_trace_proj|]; eauto.
+  Qed.
 
-Eval compute in z_to_n 0.
+  Theorem trace_on_Pair_off tg e1 e2 m
+  : (forall n, trace_proj tg (Trace_on e1 n) = empty_set')
+    -> (forall n, trace_proj tg (Trace_on e2 n) = empty_set')
+    -> trace_proj tg (Trace_on (E_Pair e1 e2) m) = empty_set'.
+  Proof.
+    intros.
+    unfold Trace_on.
+    destruct (Enumerates_from_dec _ _) as [[v t] Henum].
+    inversion Henum; subst.
+    apply Trace_on_correct in H4.
+    apply Trace_on_correct in H8.
+    simpl.
+    subst.
+    rewrite trace_proj_plus_distrl.
+    rewrite H, H0.
+    trivial.
+  Qed.
 
-Theorem z_to_n_correct n x
-: set_In x (z_to_n n) <-> x < n.
-Proof.
-  generalize dependent x.
-  induction n.
+  Theorem trace_lt_Pair_off tg e1 e2 m
+  : (forall n, trace_proj tg (Trace_on e1 n) = empty_set')
+    -> (forall n, trace_proj tg (Trace_on e2 n) = empty_set')
+    -> trace_proj tg (Trace_lt (E_Pair e1 e2) m) = empty_set'.
+  Proof.
+    induction m; [intros; destruct tg; reflexivity|].
+    intros H1 H2.
+    unfold Trace_lt; fold Trace_lt.
+    rewrite trace_proj_plus_distrl.
+    apply subset_nil_nil.
+    apply subset_union_both.
+    rewrite trace_on_Pair_off; [apply subset_refl| |]; auto.
+    rewrite IHm; auto.
+  Qed.
 
-  intros x; compute; split; [apply False_ind | intros contra; inversion contra].
-  intros x.
-  destruct (eq_nat_dec x n).
-  simpl.
-  subst.
-  split; [nliamega|].
-  intros _.
-  apply set_add_intro2; auto.
-
-  split.
-  simpl.
-  intros H.
-  assert (set_In x (z_to_n n)).
-  apply set_add_elim2 with (b := n) (Aeq_dec := eq_nat_dec); auto.
-  assert (x < n).
-  apply IHn.
-  auto.
-  nliamega.
-
-  intros H.
-  simpl.
-  apply set_add_intro1.
-  apply IHn.
-  nliamega.
-Qed.
-
-Theorem set_In_trace' (tg : tag) e x m n :
-  set_In x (trace_proj tg (Trace_from_to e m (S (m + n))))
-  <->
-  (exists k,
-     m <= k < S (m + n) /\ set_In x (trace_proj tg (Trace_on e k))).
-Proof.
-  split.
-  generalize dependent m.
-  induction n; intros m;
+  Theorem set_In_trace' (tg : tag) e x m n :
+    set_In x (trace_proj tg (Trace_from_to e m (S (m + n))))
+    <->
+    (exists k,
+       m <= k < S (m + n) /\ set_In x (trace_proj tg (Trace_on e k))).
+  Proof.
+    split.
+    generalize dependent m.
+    induction n; intros m;
     [
       replace (S (m + 0)) with (S m) by nliamega;
       destruct tg;
@@ -2006,7 +1943,7 @@ Proof.
       remember (Trace_from_to e m (m + S n)) as t; destruct t as [t0' t1' t2' t3'];
       replace (m + S n) with (S (m + n)) in * by nliamega;
       destruct tg;
-      (simpl; intros Hin_union; unfold set_union' in Hin_union;
+      (simpl; intros Hin_union;
        destruct (set_union_elim eq_nat_dec _ _ _ Hin_union);
        [exists (S (m + n)); split; [nliamega|]; destruct Heqt; auto |]);
       [ replace t0' with (trace_proj zero  (Trace_from_to e m (S (m + n)))) in H by (rewrite <-Heqt0; auto)
@@ -2016,650 +1953,621 @@ Proof.
       ];
       (destruct (IHn m H) as [k [Hless Hinn]]; exists k; (split; [nliamega | auto]))].
 
-  intros [k [[Hmk HkSmn] Hin]];
-  induction n as [| n].
-  replace (S (m + 0)) with (S m) in * by nliamega;
-  unfold Trace_from_to;
-  destruct (le_lt_dec (S m) m); [apply le_Sn_n in l; contradiction|];
-  fold Trace_from_to; rewrite trace_from_to_self; assert (k = m) by nliamega; subst;
+    intros [k [[Hmk HkSmn] Hin]];
+      induction n as [| n].
+    replace (S (m + 0)) with (S m) in * by nliamega;
+      unfold Trace_from_to;
+      destruct (le_lt_dec (S m) m); [apply le_Sn_n in l; contradiction|];
+      fold Trace_from_to; rewrite trace_from_to_self; assert (k = m) by nliamega; subst;
 
-  remember (trace_plus (Trace_on e m) trace_zero) as t;
-  destruct t; simpl in *;
-  remember (Trace_on e m) as t';
-    destruct t';
-    simpl in *;
-  inversion Heqt; subst; auto.
+      remember (trace_plus (Trace_on e m) trace_zero) as t;
+      destruct t; simpl in *;
+      remember (Trace_on e m) as t';
+      destruct t';
+      simpl in *;
+      inversion Heqt; subst; auto.
 
-  replace (S (m + n)) with (m + S n) in * by nliamega;
-  destruct (eq_nat_dec k (m + S n)); subst;
-  unfold Trace_from_to; fold Trace_from_to;
-  (destruct (le_lt_dec (S (m + S n)) m); [ assert (~ (S (m + S n) <= m)) by (apply le_not_gt; nliamega); contradiction| ]); (remember (Trace_on e (m + S n)) as t); destruct t as [t0 t1 t2 t3];
-   (remember (Trace_from_to e m (m + S n)) as t'); destruct t' as [t0' t1' t2' t3'].
-  destruct tg; (
-      simpl in *; unfold set_union'; apply set_union_intro1; auto).
+    replace (S (m + n)) with (m + S n) in * by nliamega;
+      destruct (eq_nat_dec k (m + S n)); subst;
+      unfold Trace_from_to; fold Trace_from_to;
+      (destruct (le_lt_dec (S (m + S n)) m); [ assert (~ (S (m + S n) <= m)) by (apply le_not_gt; nliamega); contradiction| ]); (remember (Trace_on e (m + S n)) as t); destruct t as [t0 t1 t2 t3];
+      (remember (Trace_from_to e m (m + S n)) as t'); destruct t' as [t0' t1' t2' t3'].
+    destruct tg; (
+        simpl in *; apply set_union_intro1; auto).
 
-  destruct tg; simpl in *; unfold set_union'; apply set_union_intro2; apply IHn; nliamega.
-Qed.
+    destruct tg; simpl in *; apply set_union_intro2; apply IHn; nliamega.
+  Qed.
 
-Theorem set_In_Trace_from_to (tg : tag) e x m n :
-  (m < n) ->
-  (set_In x (trace_proj tg (Trace_from_to e m n)) <->
-   (exists k,
-     m <= k < n /\ set_In x (trace_proj tg (Trace_on e k)))).
-Proof.
-  intros H.
-  remember (pred (n - m)) as p.
-  assert (n = (S (m + p))) by nliamega.
-  subst n.
-  apply set_In_trace'.
-Qed.
+  Theorem set_In_Trace_from_to (tg : tag) e x m n :
+    (m < n) ->
+    (set_In x (trace_proj tg (Trace_from_to e m n)) <->
+     (exists k,
+        m <= k < n /\ set_In x (trace_proj tg (Trace_on e k)))).
+  Proof.
+    intros H.
+    remember (pred (n - m)) as p.
+    assert (n = (S (m + p))) by nliamega.
+    subst n.
+    apply set_In_trace'.
+  Qed.
 
-Theorem set_In_Trace_lt tg e x n :
-set_In x (trace_proj tg (Trace_lt e (S n)))
-<->
-exists k,
-  k < S n /\ set_In x (trace_proj tg (Trace_on e k)).
-Proof.
-  destruct (set_In_Trace_from_to tg e x 0 (S n)) as [Hl Hr]; try nliamega.
-  admit.
-Qed.
-Eval compute in Trace_lt E_PairNN (S (5 * 5)).
+  Theorem set_In_Trace_lt tg e x n :
+    set_In x (trace_proj tg (Trace_lt e (S n)))
+    <->
+    exists k,
+      k < S n /\ set_In x (trace_proj tg (Trace_on e k)).
+  Proof.
+    destruct (set_In_Trace_from_to tg e x 0 (S n)) as [Hl Hr]; try nliamega.
+    admit.
+  Qed.
 
-Definition PairNN2 (k : nat)
-: trace_proj two (Trace_on E_PairNN k) = empty_set'.
-Proof.
-Admitted.
+  Theorem sub_trace_plus_introl t1 t2 t3
+  : sub_trace t1 t2 -> sub_trace t1 (trace_plus t2 t3).
+  Proof.
+    unfold sub_trace, trace_plus; destruct t1, t2, t3.
+    intros H; destruct H as [H1 [H2 [H3 H4]]].
+    Local Hint Resolve subset_union_transl.
+    split4; auto.
+  Qed.
 
-Lemma EPair_ft_cong n e1 e2 :
-    trace_eq (Trace_from_to (E_Pair e1 e2) (n * n) (S n * S n))
-             (trace_plus (Trace_lt e1 (S n))
-                         (Trace_lt e2 (S n))).
-Proof.
-  unfold trace_eq;
-  remember (Trace_from_to (E_Pair e1 e2) (n * n) (S n * S n)) as t;
-  destruct t as [t0 t1 t2 t3].
-  remember (trace_plus (Trace_lt e1 (S n)) (Trace_lt e2 (S n))) as t';
-    destruct t' as [t0' t1' t2' t3'].
-  split4; split.
-Admitted.
+  Theorem sub_trace_plus_intror t1 t2 t3
+  : sub_trace t1 t3 -> sub_trace t1 (trace_plus t2 t3).
+  Proof.
+    unfold sub_trace, trace_plus; destruct t1, t2, t3.
+    intros H; destruct H as [H1 [H2 [H3 H4]]].
+    Local Hint Resolve subset_union_transr.
+    split4; auto.
+  Qed.
 
-Theorem sub_trace_plus_introl t1 t2 t3
-: sub_trace t1 t2 -> sub_trace t1 (trace_plus t2 t3).
-Proof.
-  unfold sub_trace, trace_plus; destruct t1, t2, t3.
-  intros H; destruct H as [H1 [H2 [H3 H4]]].
-  Local Hint Resolve subset_union_transl.
-  split4; auto.
-Qed.
+  Theorem Trace_from_to_sub' e m n p : sub_trace (Trace_from_to e m n) (Trace_from_to e m (n + p)).
+  Proof.
+    induction p.
+    replace (n + 0) with n by nliamega; apply sub_trace_refl.
+    replace (n + S p) with (S (n + p)) by nliamega.
+    unfold Trace_from_to at 2; fold Trace_from_to.
+    destruct (le_lt_dec (S (n + p))).
+    replace (Trace_from_to e m n) with trace_zero; [apply sub_trace_refl|].
+    unfold Trace_from_to.
+    destruct n.
+    destruct (le_lt_dec 0 m); auto.
+    destruct (le_lt_dec (S n) m); auto; nliamega.
+    apply sub_trace_plus_intror; auto.
+  Qed.
 
-Theorem sub_trace_plus_intror t1 t2 t3
-: sub_trace t1 t3 -> sub_trace t1 (trace_plus t2 t3).
-Proof.
-  unfold sub_trace, trace_plus; destruct t1, t2, t3.
-  intros H; destruct H as [H1 [H2 [H3 H4]]].
-  Local Hint Resolve subset_union_transr.
-  split4; auto.
-Qed.
+  Theorem Trace_from_to_sub e m n p : n <= p -> sub_trace (Trace_from_to e m n) (Trace_from_to e m p).
+  Proof.
+    Local Hint Resolve Trace_from_to_sub'.
+    intros; replace p with (n + (p - n)) by nliamega; auto.
+  Qed.
 
-Theorem Trace_from_to_sub' e m n p : sub_trace (Trace_from_to e m n) (Trace_from_to e m (n + p)).
-Proof.
-  induction p.
-  replace (n + 0) with n by nliamega; apply sub_trace_refl.
-  replace (n + S p) with (S (n + p)) by nliamega.
-  unfold Trace_from_to at 2; fold Trace_from_to.
-  destruct (le_lt_dec (S (n + p))).
-  replace (Trace_from_to e m n) with trace_zero; [apply sub_trace_refl|].
-  unfold Trace_from_to.
-  destruct n.
-  destruct (le_lt_dec 0 m); auto.
-  destruct (le_lt_dec (S n) m); auto; nliamega.
-  apply sub_trace_plus_intror; auto.
-Qed.
+  Theorem Trace_lt_sub e m n : m <= n -> sub_trace (Trace_lt e m) (Trace_lt e n).
+  Proof.
+    intros H.
+    eapply sub_trace_trans; [apply trace_eq_weakenl; apply trace_lt_from_to_0_same| ].
+    eapply sub_trace_trans; [| apply trace_eq_weakenr; apply trace_lt_from_to_0_same].
+    apply Trace_from_to_sub; auto.
+  Qed.
 
-Theorem Trace_from_to_sub e m n p : n <= p -> sub_trace (Trace_from_to e m n) (Trace_from_to e m p).
-Proof.
-  Local Hint Resolve Trace_from_to_sub'.
-  intros; replace p with (n + (p - n)) by nliamega; auto.
-Qed.
+End EnumTrace.
 
-Theorem Trace_lt_sub e m n : m <= n -> sub_trace (Trace_lt e m) (Trace_lt e n).
-Proof.
-  intros H.
-  eapply sub_trace_trans; [apply trace_eq_weakenl; apply trace_lt_from_to_0_same| ].
-  eapply sub_trace_trans; [| apply trace_eq_weakenr; apply trace_lt_from_to_0_same].
-  apply Trace_from_to_sub; auto.
-Qed.
+Section Fairness.
+  Definition Fair2 (k : Enum -> Enum -> Enum) :=
+    forall n,
+    exists equilibrium,
+      match Trace_lt (k (E_Trace zero E_Nat) (E_Trace one E_Nat)) equilibrium with
+        | Tracing l_uses r_uses _ _ =>
+          n < equilibrium /\ set_eq  l_uses r_uses
+      end.
 
-Lemma PairNN_layer :
-  forall n,
-    trace_eq (Trace_from_to E_PairNN (n * n) (S n * S n))
-             (Tracing (z_to_n (S n)) (z_to_n (S n)) empty_set' empty_set').
-Proof.
-  intros n;
-    unfold trace_eq;
-    remember (Trace_from_to E_PairNN (n * n) (S n * S n)) as t;
-    destruct t as [t0 t1 t2 t3].
-  split4; split.
+  Definition Fair3 (k : Enum -> Enum -> Enum -> Enum) :=
+    forall n,
+    exists equilibrium,
+      match Trace_lt (k (E_Trace zero E_Nat) (E_Trace one E_Nat) (E_Trace two E_Nat)) equilibrium with
+        | Tracing z_uses o_uses t_uses _ =>
+          n < equilibrium /\ set_eq z_uses o_uses /\ set_eq o_uses t_uses
+      end.
 
-  (* Case 1: trace_left pair n^2 (n+1)^2 < 0..n+1 *)
-  apply subset_In_def;
-    assert (t0 = (trace_proj zero (Trace_from_to E_PairNN (n * n) (S n * S n)))) by (rewrite <-Heqt; auto);
-    intros x Hin;
-    apply z_to_n_correct;
-    rewrite H in Hin;
-    (apply (set_In_Trace_from_to zero) in Hin; [| nliamega]);
-    destruct Hin as [k [Hksize Hin]];
-    clear Heqt H;
-    unfold Trace_on in Hin;
-    destruct (Enumerates_from_dec E_PairNN k) as [[v t] Henum];
-    destruct (le_lt_dec (sqrt k) (k - (sqrt k * sqrt k))).
-  assert (Enumerates E_PairNN
-                     k
-                     (V_Pair (V_Nat (sqrt k)) (V_Nat ((k - sqrt k * sqrt k) - sqrt k)))
-                     (trace_plus (trace_one (sqrt k)                         zero)
-                                 (trace_one ((k - sqrt k * sqrt k) - sqrt k) one)
-                     )).
+  Definition Fair4 (k : Enum -> Enum -> Enum -> Enum -> Enum) :=
+    forall n,
+    exists equilibrium,
+      match Trace_lt (k (E_Trace zero E_Nat) (E_Trace one E_Nat) (E_Trace two E_Nat) (E_Trace three E_Nat)) equilibrium with
+        | Tracing z_uses o_uses tw_uses th_uses =>
+          n < equilibrium /\ set_eq z_uses o_uses /\ set_eq o_uses tw_uses /\ set_eq tw_uses th_uses
+      end.
 
-  apply ES_Pair with (ln := (sqrt k)) (rn := ((k - sqrt k * sqrt k) - sqrt k));
-    [| econstructor; constructor
-     | econstructor; constructor
-    ];
-    assert (k = (sqrt k * sqrt k) + sqrt k + ((k - sqrt k * sqrt k) - sqrt k)) as Hk by nliamega;
-    rewrite Hk at 1;
-    constructor;
-    apply sqrt_lemma.
-  destruct (Enumerates_from_fun _ _ _ _ _ _ Henum H); subst;
-    destruct Hin; [nliamega | contradiction].
+  Section SumFair.
+    Lemma Sum_Parity_Trace :
+      forall n,
+        Trace_on (E_Sum (E_Trace zero E_Nat) (E_Trace one E_Nat)) n
+        = trace_one (div2 n)
+                    (if even_odd_dec n
+                     then zero
+                     else one).
+    Proof.
+      intros n.
+      remember (even_odd_dec n) as mH.
+      unfold Trace_on; simpl.
+      destruct mH; rewrite <-HeqmH; auto.
+    Qed.
 
-  assert (Enumerates E_PairNN
-                     k
-                     (V_Pair (V_Nat (k - (sqrt k * sqrt k)))
-                             (V_Nat (sqrt k)))
-                     (trace_plus (trace_one (k - (sqrt k * sqrt k)) zero)
-                                 (trace_one (sqrt k)                one))).
-  apply ES_Pair with (ln := (k - (sqrt k * sqrt k))) (rn := sqrt k);
-    [ rewrite (sqrt_lemma' k) at 1; [constructor; auto | auto]
-    | econstructor; constructor
-    | econstructor; constructor ].
-  destruct (Enumerates_from_fun _ _ _ _ _ _ Henum H); subst;
-    destruct Hin; [nliamega | contradiction].
+    (* Proof idea: equilibrium = 2 * n + 2,  uses = 0..(S n) *)
+    Theorem Sum_Fair : Fair2 E_Sum.
+    Proof.
+      unfold Fair2.
+      intros n.
+      exists (2 * n + 2).
+      remember (Trace_lt (E_Sum (E_Trace zero E_Nat) (E_Trace one E_Nat)) (2 * n + 2)).
+      destruct t as [tz to ttw tth].
+      split; [nliamega| ].
 
-  (* Case 2: 0..n+1 < trace_left pair n^2 (n+1)^2 *)
-  apply subset_In_def;
-    intros x Hin;
-    apply z_to_n_correct in Hin;
-    assert (t0 = (trace_proj zero (Trace_from_to E_PairNN (n * n) (S n * S n)))) by (rewrite <-Heqt; auto);
-    rewrite H;
-    (apply (set_In_Trace_from_to zero); [nliamega| ]);
-  (* our k is (unpair x n)
-   *)
-    destruct (le_lt_dec n x).
+      generalize dependent tth.
+      generalize dependent ttw.
+      generalize dependent to.
+      generalize dependent tz.
+      induction n.
+      intros tz to ttw tth Heqt.
+      inversion Heqt; auto; apply set_eq_refl.
 
-  exists (x*x + x + n); split; [nliamega|];
-    unfold Trace_on;
-    destruct (Enumerates_from_dec E_PairNN (x * x + x + n)) as [[v t] Henum];
-    assert (Enumerates E_PairNN
-                     (x * x + x + n)
-                     (V_Pair (V_Nat x) (V_Nat n))
-                     (trace_plus (trace_one x zero) (trace_one n one))).
-  econstructor;
-    [ constructor 1; auto
-    | econstructor; constructor
-    | econstructor; constructor
-    ].
-  destruct (Enumerates_from_fun _ _ _ _ _ _ Henum H0); subst; simpl; tauto.
+      intros tz to ttw tth Htzto.
+      remember (Trace_lt (E_Sum (E_Trace zero E_Nat) (E_Trace one E_Nat)) (2 * n + 2)).
+      replace (2 * S n + 2) with (S (S (2 * n + 2))) in Htzto by nliamega.
+      simpl in Htzto.
+      replace (n + (n + 0) + 2) with (2 * n + 2) in Htzto by nliamega.
+      destruct t as [tz' to' ttw' tth'].
+      assert (set_eq tz' to').
+      eapply IHn ; auto.
+      rewrite <-Heqt in Htzto.
+      clear Heqt.
+      clear IHn.
+      replace (Trace_on (E_Sum (E_Trace zero E_Nat) (E_Trace one E_Nat)) (S (2 * n + 2))) with (trace_one (S n) one) in Htzto.
 
-  exists (x + n * n); split; [nliamega|];
-    unfold Trace_on;
-    destruct (Enumerates_from_dec E_PairNN (x + n * n)) as [[v t] Henum];
-    assert (Enumerates E_PairNN
-                       (x + n * n)
-                       (V_Pair (V_Nat x) (V_Nat n))
-                       (trace_plus (trace_one x zero) (trace_one n one))).
-  econstructor;
-    [ constructor 2; auto
-    | econstructor; constructor
-    | econstructor; constructor ].
-  destruct (Enumerates_from_fun _ _ _ _ _ _ Henum H0); subst; simpl; tauto.
+      replace (Trace_on (E_Sum (E_Trace zero E_Nat) (E_Trace one E_Nat)) ((2 * n)+2)) with (trace_one (S n) zero) in Htzto.
+      unfold trace_one in Htzto.
+      unfold trace_plus in Htzto.
+      inversion Htzto.
+      clear  Htzto H1 H2.
 
-  (* this half of the proof is almost exactly the same as above,
+      - SearchAbout set_eq.
+        apply set_eq_trans with (s2 := set_union' (S n :: nil) tz').
+        apply set_union_unitl.
+        apply set_eq_trans with (s2 := set_union' (S n :: nil) to').
+        apply set_union_cong; auto.
+        apply set_union_cong.
+        apply set_eq_refl.
+        apply set_eq_symm.
+        apply set_union_unitl.
+
+      (* Trace (left + right) (2n+3) =  *)
+      - unfold Trace_on.
+        destruct (Enumerates_from_dec (E_Sum (E_Trace zero E_Nat) (E_Trace one E_Nat)) (2 * n + 2)).
+        assert (Enumerates (E_Sum (E_Trace zero E_Nat) (E_Trace one E_Nat)) (2 * n + 2) (V_Sum_Left (V_Nat (S n))) (trace_one (S n) zero)).
+        apply ES_Sum_Left with (ln := (S n)); [nliamega| ].
+        econstructor.
+        constructor.
+        destruct x.
+
+        destruct (Enumerates_from_fun _ _ _ _ _ _ y H0); subst.
+        auto.
+
+      - unfold Trace_on.
+        destruct (Enumerates_from_dec (E_Sum (E_Trace zero E_Nat) (E_Trace one E_Nat)) (S (2 * n + 2))).
+        assert (Enumerates (E_Sum (E_Trace zero E_Nat) (E_Trace one E_Nat)) (S (2 * n + 2)) (V_Sum_Right (V_Nat (S n))) (trace_one (S n) one)).
+        apply ES_Sum_Right with (rn := S n); [nliamega|].
+        econstructor; constructor.
+        destruct x.
+        destruct (Enumerates_from_fun _ _ _ _ _ _ y H0); subst.
+        auto.
+    Qed.
+
+    Eval compute in (Trace_lt (E_Pair (E_Trace zero E_Nat) (E_Trace one E_Nat)) 64).
+  End SumFair.
+
+  Section PairFair.
+    Definition E_PairNN := (E_Pair (E_Trace zero E_Nat) (E_Trace one E_Nat)).
+    Lemma PairNN_layer :
+      forall n,
+        trace_eq (Trace_from_to E_PairNN (n * n) (S n * S n))
+                 (Tracing (z_to_n (S n)) (z_to_n (S n)) empty_set' empty_set').
+    Proof.
+      intros n;
+      unfold trace_eq;
+      remember (Trace_from_to E_PairNN (n * n) (S n * S n)) as t;
+      destruct t as [t0 t1 t2 t3].
+      split4; split.
+
+      (* Case 1: trace_left pair n^2 (n+1)^2 < 0..n+1 *)
+      apply subset_In_def;
+        assert (t0 = (trace_proj zero (Trace_from_to E_PairNN (n * n) (S n * S n)))) by (rewrite <-Heqt; auto);
+        intros x Hin;
+        apply z_to_n_correct;
+        rewrite H in Hin;
+        (apply (set_In_Trace_from_to zero) in Hin; [| nliamega]);
+        destruct Hin as [k [Hksize Hin]];
+        clear Heqt H;
+        unfold Trace_on in Hin;
+        destruct (Enumerates_from_dec E_PairNN k) as [[v t] Henum];
+        destruct (le_lt_dec (sqrt k) (k - (sqrt k * sqrt k))).
+      assert (Enumerates E_PairNN
+                         k
+                         (V_Pair (V_Nat (sqrt k)) (V_Nat ((k - sqrt k * sqrt k) - sqrt k)))
+                         (trace_plus (trace_one (sqrt k)                         zero)
+                                     (trace_one ((k - sqrt k * sqrt k) - sqrt k) one)
+             )).
+
+      apply ES_Pair with (ln := (sqrt k)) (rn := ((k - sqrt k * sqrt k) - sqrt k));
+        [| econstructor; constructor
+         | econstructor; constructor
+        ];
+        assert (k = (sqrt k * sqrt k) + sqrt k + ((k - sqrt k * sqrt k) - sqrt k)) as Hk by nliamega;
+        rewrite Hk at 1;
+        constructor;
+        apply sqrt_lemma.
+      destruct (Enumerates_from_fun _ _ _ _ _ _ Henum H); subst;
+      destruct Hin; [nliamega | contradiction].
+
+      assert (Enumerates E_PairNN
+                         k
+                         (V_Pair (V_Nat (k - (sqrt k * sqrt k)))
+                                 (V_Nat (sqrt k)))
+                         (trace_plus (trace_one (k - (sqrt k * sqrt k)) zero)
+                                     (trace_one (sqrt k)                one))).
+      apply ES_Pair with (ln := (k - (sqrt k * sqrt k))) (rn := sqrt k);
+        [ rewrite (sqrt_lemma' k) at 1; [constructor; auto | auto]
+        | econstructor; constructor
+        | econstructor; constructor ].
+      destruct (Enumerates_from_fun _ _ _ _ _ _ Henum H); subst;
+      destruct Hin; [nliamega | contradiction].
+
+      (* Case 2: 0..n+1 < trace_left pair n^2 (n+1)^2 *)
+      apply subset_In_def;
+        intros x Hin;
+        apply z_to_n_correct in Hin;
+        assert (t0 = (trace_proj zero (Trace_from_to E_PairNN (n * n) (S n * S n)))) by (rewrite <-Heqt; auto);
+        rewrite H;
+        (apply (set_In_Trace_from_to zero); [nliamega| ]);
+        (* our k is (unpair x n)
+         *)
+        destruct (le_lt_dec n x).
+
+      exists (x*x + x + n); split; [nliamega|];
+      unfold Trace_on;
+      destruct (Enumerates_from_dec E_PairNN (x * x + x + n)) as [[v t] Henum];
+      assert (Enumerates E_PairNN
+                         (x * x + x + n)
+                         (V_Pair (V_Nat x) (V_Nat n))
+                         (trace_plus (trace_one x zero) (trace_one n one))).
+      econstructor;
+        [ constructor 1; auto
+        | econstructor; constructor
+        | econstructor; constructor
+        ].
+      destruct (Enumerates_from_fun _ _ _ _ _ _ Henum H0); subst; simpl; tauto.
+
+      exists (x + n * n); split; [nliamega|];
+      unfold Trace_on;
+      destruct (Enumerates_from_dec E_PairNN (x + n * n)) as [[v t] Henum];
+      assert (Enumerates E_PairNN
+                         (x + n * n)
+                         (V_Pair (V_Nat x) (V_Nat n))
+                         (trace_plus (trace_one x zero) (trace_one n one))).
+      econstructor;
+        [ constructor 2; auto
+        | econstructor; constructor
+        | econstructor; constructor ].
+      destruct (Enumerates_from_fun _ _ _ _ _ _ Henum H0); subst; simpl; tauto.
+
+      (* this half of the proof is almost exactly the same as above,
      except with t1 instead of t0 should figure how to be less
      repetitive than repeating all the above tactics.  might be less
      of a problem when we move to a new trace representation
-   *)
-  (* Case 3: trace_right pair n^2 (n+1)^2 < 0..n+1 *)
-  apply subset_In_def;
-    assert (t1 = (trace_proj one (Trace_from_to E_PairNN (n * n) (S n * S n)))) by (rewrite <-Heqt; auto);
-    intros x Hin;
-    apply z_to_n_correct;
-    rewrite H in Hin;
-    (apply (set_In_Trace_from_to one) in Hin; [| nliamega]);
-    destruct Hin as [k [Hksize Hin]];
-    clear Heqt H;
-    unfold Trace_on in Hin;
-    destruct (Enumerates_from_dec E_PairNN k) as [[v t] Henum].
-    destruct (le_lt_dec (sqrt k) (k - (sqrt k * sqrt k))).
-  assert (Enumerates E_PairNN
-                     k
-                     (V_Pair (V_Nat (sqrt k)) (V_Nat ((k - sqrt k * sqrt k) - sqrt k)))
-                     (trace_plus (trace_one (sqrt k)                         zero)
-                                 (trace_one ((k - sqrt k * sqrt k) - sqrt k) one)
-                     )).
+       *)
+      (* Case 3: trace_right pair n^2 (n+1)^2 < 0..n+1 *)
+      apply subset_In_def;
+        assert (t1 = (trace_proj one (Trace_from_to E_PairNN (n * n) (S n * S n)))) by (rewrite <-Heqt; auto);
+        intros x Hin;
+        apply z_to_n_correct;
+        rewrite H in Hin;
+        (apply (set_In_Trace_from_to one) in Hin; [| nliamega]);
+        destruct Hin as [k [Hksize Hin]];
+        clear Heqt H;
+        unfold Trace_on in Hin;
+        destruct (Enumerates_from_dec E_PairNN k) as [[v t] Henum].
+      destruct (le_lt_dec (sqrt k) (k - (sqrt k * sqrt k))).
+      assert (Enumerates E_PairNN
+                         k
+                         (V_Pair (V_Nat (sqrt k)) (V_Nat ((k - sqrt k * sqrt k) - sqrt k)))
+                         (trace_plus (trace_one (sqrt k)                         zero)
+                                     (trace_one ((k - sqrt k * sqrt k) - sqrt k) one)
+             )).
 
-  apply ES_Pair with (ln := (sqrt k)) (rn := ((k - sqrt k * sqrt k) - sqrt k));
-    [| econstructor; constructor
-     | econstructor; constructor
-    ];
-    assert (k = (sqrt k * sqrt k) + sqrt k + ((k - sqrt k * sqrt k) - sqrt k)) as Hk by nliamega;
-    rewrite Hk at 1;
-    constructor;
-    apply sqrt_lemma.
-  destruct (Enumerates_from_fun _ _ _ _ _ _ Henum H); subst;
-    destruct Hin;
-    [ rewrite <- H0; apply sqrt_lemma''; auto
-    | contradiction].
+      apply ES_Pair with (ln := (sqrt k)) (rn := ((k - sqrt k * sqrt k) - sqrt k));
+        [| econstructor; constructor
+         | econstructor; constructor
+        ];
+        assert (k = (sqrt k * sqrt k) + sqrt k + ((k - sqrt k * sqrt k) - sqrt k)) as Hk by nliamega;
+        rewrite Hk at 1;
+        constructor;
+        apply sqrt_lemma.
+      destruct (Enumerates_from_fun _ _ _ _ _ _ Henum H); subst;
+      destruct Hin;
+      [ rewrite <- H0; apply sqrt_lemma''; auto
+      | contradiction].
 
-  assert (Enumerates E_PairNN
-                     k
-                     (V_Pair (V_Nat (k - (sqrt k * sqrt k)))
-                             (V_Nat (sqrt k)))
-                     (trace_plus (trace_one (k - (sqrt k * sqrt k)) zero)
-                                 (trace_one (sqrt k)                one))).
-  apply ES_Pair with (ln := (k - (sqrt k * sqrt k))) (rn := sqrt k);
-    [ rewrite (sqrt_lemma' k) at 1; [constructor; auto | auto]
-    | econstructor; constructor
-    | econstructor; constructor ].
-  destruct (Enumerates_from_fun _ _ _ _ _ _ Henum H); subst;
-  destruct Hin;
-  [ rewrite <-H0; rewrite (Nat.sqrt_unique k n); nliamega
-  | contradiction
-  ].
+      assert (Enumerates E_PairNN
+                         k
+                         (V_Pair (V_Nat (k - (sqrt k * sqrt k)))
+                                 (V_Nat (sqrt k)))
+                         (trace_plus (trace_one (k - (sqrt k * sqrt k)) zero)
+                                     (trace_one (sqrt k)                one))).
+      apply ES_Pair with (ln := (k - (sqrt k * sqrt k))) (rn := sqrt k);
+        [ rewrite (sqrt_lemma' k) at 1; [constructor; auto | auto]
+        | econstructor; constructor
+        | econstructor; constructor ].
+      destruct (Enumerates_from_fun _ _ _ _ _ _ Henum H); subst;
+      destruct Hin;
+      [ rewrite <-H0; rewrite (Nat.sqrt_unique k n); nliamega
+      | contradiction
+      ].
 
-  (* Case 4: 0..n+1 < trace_right pair n^2 (n+1)^2 *)
-  apply subset_In_def;
-    intros x Hin;
-    apply z_to_n_correct in Hin;
-    assert (t1 = (trace_proj one (Trace_from_to E_PairNN (n * n) (S n * S n)))) by (rewrite <-Heqt; auto);
-    rewrite H;
-    (apply (set_In_Trace_from_to one); [nliamega| ]);
-    destruct (le_lt_dec x n).
-  exists (n * n + n + x); split; [nliamega | ];
-    unfold Trace_on;
-    destruct (Enumerates_from_dec E_PairNN (n * n + n + x)) as [[v t] Henum];
-    assert (Enumerates E_PairNN
-                     (n * n + n + x)
-                     (V_Pair (V_Nat n) (V_Nat x))
-                     (trace_plus (trace_one n zero) (trace_one x one))).
-  econstructor;
-    [ constructor 1; auto
-    | econstructor; constructor
-    | econstructor; constructor
-    ].
-  destruct (Enumerates_from_fun _ _ _ _ _ _ Henum H0); subst; simpl; tauto.
+      (* Case 4: 0..n+1 < trace_right pair n^2 (n+1)^2 *)
+      apply subset_In_def;
+        intros x Hin;
+        apply z_to_n_correct in Hin;
+        assert (t1 = (trace_proj one (Trace_from_to E_PairNN (n * n) (S n * S n)))) by (rewrite <-Heqt; auto);
+        rewrite H;
+        (apply (set_In_Trace_from_to one); [nliamega| ]);
+        destruct (le_lt_dec x n).
+      exists (n * n + n + x); split; [nliamega | ];
+      unfold Trace_on;
+      destruct (Enumerates_from_dec E_PairNN (n * n + n + x)) as [[v t] Henum];
+      assert (Enumerates E_PairNN
+                         (n * n + n + x)
+                         (V_Pair (V_Nat n) (V_Nat x))
+                         (trace_plus (trace_one n zero) (trace_one x one))).
+      econstructor;
+        [ constructor 1; auto
+        | econstructor; constructor
+        | econstructor; constructor
+        ].
+      destruct (Enumerates_from_fun _ _ _ _ _ _ Henum H0); subst; simpl; tauto.
 
-  exists (n + x * x); split; [nliamega| ];
-    unfold Trace_on;
-    destruct (Enumerates_from_dec E_PairNN (n + x * x)) as [[v t] Henum];
-    assert (Enumerates E_PairNN
-                     (n + x * x)
-                     (V_Pair (V_Nat n) (V_Nat x))
-                     (trace_plus (trace_one n zero) (trace_one x one))).
-  econstructor;
-    [ constructor 2; auto
-    | econstructor; constructor
-    | econstructor; constructor
-    ].
-  destruct (Enumerates_from_fun _ _ _ _ _ _ Henum H0); subst; simpl; tauto.
+      exists (n + x * x); split; [nliamega| ];
+      unfold Trace_on;
+      destruct (Enumerates_from_dec E_PairNN (n + x * x)) as [[v t] Henum];
+      assert (Enumerates E_PairNN
+                         (n + x * x)
+                         (V_Pair (V_Nat n) (V_Nat x))
+                         (trace_plus (trace_one n zero) (trace_one x one))).
+      econstructor;
+        [ constructor 2; auto
+        | econstructor; constructor
+        | econstructor; constructor
+        ].
+      destruct (Enumerates_from_fun _ _ _ _ _ _ Henum H0); subst; simpl; tauto.
 
-  unfold empty_set', empty_set, E_PairNN in *;
-    replace t2 with (trace_proj two (Trace_from_to (E_Pair (E_Trace zero E_Nat) (E_Trace one E_Nat))
-                                                 (n * n) (S n * S n)))
-    by (rewrite <-Heqt; trivial);
-    apply subset_trans with (s2 := (trace_proj two (Trace_lt (E_Pair (E_Trace zero E_Nat) (E_Trace one E_Nat))
-                                                             (S n * S n)))).
-  (eapply subset_trans;
-    [|apply set_subset_weaken; apply trace_eq_proj; apply trace_eq_symm; apply trace_lt_from_to_0_same]);
-  apply sub_trace_proj; apply sub_trace_from_to; nliamega.
-  rewrite trace_lt_Pair_off; auto.
-  
-  apply subset_nil.
+      unfold empty_set, E_PairNN in *;
+        replace t2 with (trace_proj two (Trace_from_to (E_Pair (E_Trace zero E_Nat) (E_Trace one E_Nat))
+                                                       (n * n) (S n * S n)))
+        by (rewrite <-Heqt; trivial);
+        apply subset_trans with (s2 := (trace_proj two (Trace_lt (E_Pair (E_Trace zero E_Nat) (E_Trace one E_Nat))
+                                                                 (S n * S n)))).
+      (eapply subset_trans;
+       [|apply set_subset_weaken; apply trace_eq_proj; apply trace_eq_symm; apply trace_lt_from_to_0_same]);
+        apply sub_trace_proj; apply sub_trace_from_to; nliamega.
+      rewrite trace_lt_Pair_off; auto.
+      
+      apply subset_nil.
 
-  unfold empty_set', empty_set, E_PairNN in *;
-    replace t3 with (trace_proj three (Trace_from_to (E_Pair (E_Trace zero E_Nat) (E_Trace one E_Nat))
-                                                 (n * n) (S n * S n)))
-    by (rewrite <-Heqt; trivial);
-    apply subset_trans with (s2 := (trace_proj three (Trace_lt (E_Pair (E_Trace zero E_Nat) (E_Trace one E_Nat))
-                                                             (S n * S n)))).
-  (eapply subset_trans;
-    [|apply set_subset_weaken; apply trace_eq_proj; apply trace_eq_symm; apply trace_lt_from_to_0_same]);
-  apply sub_trace_proj; apply sub_trace_from_to; nliamega.
-  rewrite trace_lt_Pair_off; auto.
+      unfold empty_set, E_PairNN in *;
+        replace t3 with (trace_proj three (Trace_from_to (E_Pair (E_Trace zero E_Nat) (E_Trace one E_Nat))
+                                                         (n * n) (S n * S n)))
+        by (rewrite <-Heqt; trivial);
+        apply subset_trans with (s2 := (trace_proj three (Trace_lt (E_Pair (E_Trace zero E_Nat) (E_Trace one E_Nat))
+                                                                   (S n * S n)))).
+      (eapply subset_trans;
+       [|apply set_subset_weaken; apply trace_eq_proj; apply trace_eq_symm; apply trace_lt_from_to_0_same]);
+        apply sub_trace_proj; apply sub_trace_from_to; nliamega.
+      rewrite trace_lt_Pair_off; auto.
 
-  apply subset_nil.
-Qed.
+      apply subset_nil.
+    Qed.
 
-Lemma Pair_precise
-: forall n e1 e2,
-    trace_eq (Trace_lt (E_Pair e1 e2) (n * n))
-             (trace_plus (Trace_lt e1 n)
-                         (Trace_lt e2 n)).
-  intros n.
-  induction n as [| n IHn]; [  intros; compute; tauto| ].
-  intros e1 e2.
-  eapply trace_eq_trans.
-  apply trace_from_to_0_split with (m := n * n) (n := S n * S n); nliamega.
-  admit.
-Qed.
+    Lemma EPair_ft_cong n e1 e2 :
+      trace_eq (Trace_from_to (E_Pair e1 e2) (n * n) (S n * S n))
+               (trace_plus (Trace_lt e1 (S n))
+                           (Trace_lt e2 (S n))).
+    Proof.
+      unfold trace_eq;
+      remember (Trace_from_to (E_Pair e1 e2) (n * n) (S n * S n)) as t;
+      destruct t as [t0 t1 t2 t3].
+      remember (trace_plus (Trace_lt e1 (S n)) (Trace_lt e2 (S n))) as t';
+        destruct t' as [t0' t1' t2' t3'].
+      split4; split.
+    Admitted.
 
-Lemma PairPair_precise
-: forall n e1 e2 e3,
-    trace_eq (Trace_lt (E_Pair e1 (E_Pair e2 e3)) ((n * n) * (n * n)))
-             (trace_plus (Trace_lt e1 (n * n))
-                         (trace_plus (Trace_lt e2 n)
-                                     (Trace_lt e3 n))).
-Proof.
-  intros n e1 e2 e3.
-  eapply trace_eq_trans; [apply Pair_precise|].
-  apply trace_plus_cong; [apply trace_eq_refl| ].
-  apply Pair_precise.
-Qed.
+    Lemma Pair_precise
+    : forall n e1 e2,
+        trace_eq (Trace_lt (E_Pair e1 e2) (n * n))
+                 (trace_plus (Trace_lt e1 n)
+                             (Trace_lt e2 n)).
+      intros n.
+      induction n as [| n IHn]; [  intros; compute; tauto| ].
+      intros e1 e2.
+      eapply trace_eq_trans.
+      apply trace_from_to_0_split with (m := n * n) (n := S n * S n); nliamega.
+      admit.
+    Qed.
 
-Definition foobar n := ((S (sqrt (S (sqrt n)))) * (S (sqrt (S (sqrt n))))) * ((S (sqrt (S (sqrt n)))) * (S (sqrt (S (sqrt n))))).
-Definition qux n := S (S (sqrt (S (sqrt n)))) * S (S (sqrt (S (sqrt n)))).
-Definition baz n := (qux n, n, foobar n).
-Eval compute in baz 0.
-Eval compute in baz 1.
-Eval compute in baz 2.
-Eval compute in baz 3.
-Eval compute in baz 4.
-Eval compute in baz 5.
-Eval compute in baz 6.
-Eval compute in baz 7.
-Eval compute in baz 8.
-Eval compute in baz 9.
-Eval compute in baz 10.
-Eval compute in baz 11.
-Eval compute in baz 12.
-Eval compute in baz 13.
-Eval compute in baz 14.
-Eval compute in baz 15.
-Eval compute in baz 16.
-Eval compute in baz 17.
-Eval compute in baz 25.
-Eval compute in baz 36.
-Eval compute in baz 49.
-Eval compute in baz 100.
+    Lemma PairPair_precise
+    : forall n e1 e2 e3,
+        trace_eq (Trace_lt (E_Pair e1 (E_Pair e2 e3)) ((n * n) * (n * n)))
+                 (trace_plus (Trace_lt e1 (n * n))
+                             (trace_plus (Trace_lt e2 n)
+                                         (Trace_lt e3 n))).
+    Proof.
+      intros n e1 e2 e3.
+      eapply trace_eq_trans; [apply Pair_precise|].
+      apply trace_plus_cong; [apply trace_eq_refl| ].
+      apply Pair_precise.
+    Qed.
 
+    Lemma Pair_Fair_precise :
+      forall n, trace_eq (Trace_lt E_PairNN (n * n)) (Tracing (z_to_n n) (z_to_n n) empty_set' empty_set').
+    Proof.
+      induction n.
+      compute; tauto.
+      apply trace_eq_trans
+      with (t2 := (trace_plus (Trace_lt E_PairNN (n * n))
+                              (Trace_from_to E_PairNN (n * n) (S n * S n)))).
+      apply trace_from_to_0_split; nliamega.
+      apply trace_eq_trans with (t2 := (trace_plus (Tracing (z_to_n n) (z_to_n n) empty_set' empty_set')
+                                                   (Tracing (z_to_n (S n)) (z_to_n (S n)) empty_set' empty_set'))).
+      apply trace_plus_cong; auto.
+      apply PairNN_layer.
+      apply trace_eq_trans with (t2 := (Tracing (z_to_n (S n)) (z_to_n (S n))) empty_set' empty_set').
+      unfold trace_eq.
+      split4;
+        [ (apply subset_union_eq; unfold z_to_n at 2; fold z_to_n; apply set_subset_add; apply subset_refl)
+        | (apply subset_union_eq; unfold z_to_n at 2; fold z_to_n; apply set_subset_add; apply subset_refl)
+        | apply set_eq_refl
+        | apply set_eq_refl ].
 
-Lemma mult_lt_compat : forall m n p q, m < p -> n < q -> m * n < p * q.
-Proof.
-  intros; nliamega.
-Qed.
+      apply trace_eq_refl.
+    Qed.
 
+    Theorem Pair_Fair : Fair2 E_Pair.
+      unfold Fair2.
+      intros n.
+      exists ((S n) * (S n)).
 
-Lemma Pair_Fair_precise :
-  forall n, trace_eq (Trace_lt E_PairNN (n * n)) (Tracing (z_to_n n) (z_to_n n) empty_set' empty_set').
-Proof.
-  induction n.
-  compute; tauto.
-  apply trace_eq_trans
-  with (t2 := (trace_plus (Trace_lt E_PairNN (n * n))
-                          (Trace_from_to E_PairNN (n * n) (S n * S n)))).
-  apply trace_from_to_0_split; nliamega.
-  apply trace_eq_trans with (t2 := (trace_plus (Tracing (z_to_n n) (z_to_n n) empty_set' empty_set')
-                                               (Tracing (z_to_n (S n)) (z_to_n (S n)) empty_set' empty_set'))).
-  apply trace_plus_cong; auto.
-  apply PairNN_layer.
-  apply trace_eq_trans with (t2 := (Tracing (z_to_n (S n)) (z_to_n (S n))) empty_set' empty_set').
-  unfold trace_eq.
-  split4;
-    [ (apply subset_union_eq; unfold z_to_n at 2; fold z_to_n; apply set_subset_add; apply subset_refl)
-    | (apply subset_union_eq; unfold z_to_n at 2; fold z_to_n; apply set_subset_add; apply subset_refl)
-    | apply set_eq_refl
-    | apply set_eq_refl ].
+      fold E_PairNN.
+      remember (Trace_lt E_PairNN (S n * S n)) as t.
+      destruct t as [t0 t1 t2 t3].
+      split; [nliamega|].
+      remember (Pair_Fair_precise (S n)) as Hteq; clear HeqHteq.
+      unfold trace_eq in Hteq.
+      remember (Trace_lt E_PairNN (S n * S n)) as t'.
+      destruct t'.
+      inversion Heqt; subst s s0.
+      destruct4 Hteq.
+      eapply set_eq_trans; [| apply set_eq_symm]; eauto.
+    Qed.
+  End PairFair.
 
-  apply trace_eq_refl.
-Qed.
+  Section NaivePairUnfair.
 
-Theorem Pair_Fair : Fair2 E_Pair.
-  unfold Fair2.
-  intros n.
-  exists ((S n) * (S n)).
+    Definition NaivePair3 e1 e2 e3 :=
+      E_Pair e1 (E_Pair e2 e3).
 
-  fold E_PairNN.
-  remember (Trace_lt E_PairNN (S n * S n)) as t.
-  destruct t as [t0 t1 t2 t3].
-  split; [nliamega|].
-  remember (Pair_Fair_precise (S n)) as Hteq; clear HeqHteq.
-  unfold trace_eq in Hteq.
-  remember (Trace_lt E_PairNN (S n * S n)) as t'.
-  destruct t'.
-  inversion Heqt; subst s s0.
-  destruct4 Hteq.
-  eapply set_eq_trans; [| apply set_eq_symm]; eauto.
-Qed.
+    Definition AltUnfair3 k :=
+      exists threshold,
+        forall eq_cand,
+          eq_cand > threshold ->
+          match Trace_lt (k (E_Trace zero E_Nat) (E_Trace one E_Nat) (E_Trace two E_Nat)) eq_cand with
+            | Tracing use0 use1 use2 _ =>
+              (~ (set_eq use0 use1)) \/ (~ (set_eq use1 use2)) \/ (~ (set_eq use0 use2))
+          end.
 
-(* Next: prove (cons e1 (cons e2 e3)) is unfair *)
-Definition NaivePair3 e1 e2 e3 :=
-  E_Pair e1 (E_Pair e2 e3).
+    Theorem AltUnfair3Suff k : AltUnfair3 k -> ~ (Fair3 k).
+    Proof.
+      unfold AltUnfair3, Fair3, not.
+      intros [thresh Halt] Hunf.
+      destruct (Hunf thresh) as [eq_cand Hblah].
+      clear Hunf.
+      remember (Halt eq_cand).
+      clear Halt Heqy.
+      destruct (Trace_lt (k (E_Trace zero E_Nat) (E_Trace one E_Nat) (E_Trace two E_Nat))
+                         eq_cand) as [t0 t1 t2 t3] in *.
+      intuition.
+      assert (set_eq t0 t2) by (eapply set_eq_trans; eauto); contradiction.
+    Qed.
 
-Definition AltUnfair3 k :=
-  exists threshold,
-    forall eq_cand,
-      eq_cand > threshold ->
-      match Trace_lt (k (E_Trace zero E_Nat) (E_Trace one E_Nat) (E_Trace two E_Nat)) eq_cand with
-        | Tracing use0 use1 use2 _ =>
-          (~ (set_eq use0 use1)) \/ (~ (set_eq use1 use2)) \/ (~ (set_eq use0 use2))
-      end.
+    Definition traceNP3 := Trace_lt (NaivePair3 (E_Trace zero E_Nat) (E_Trace one E_Nat) (E_Trace two E_Nat)).
 
-Theorem AltUnfair3Suff k : AltUnfair3 k -> ~ (Fair3 k).
-Proof.
-  unfold AltUnfair3, Fair3, not.
-  intros [thresh Halt] Hunf.
-  destruct (Hunf thresh) as [eq_cand Hblah].
-  clear Hunf.
-  remember (Halt eq_cand).
-  clear Halt Heqy.
-  destruct (Trace_lt (k (E_Trace zero E_Nat) (E_Trace one E_Nat) (E_Trace two E_Nat))
-                            eq_cand) as [t0 t1 t2 t3] in *.
-  intuition.
-  assert (set_eq t0 t2) by (eapply set_eq_trans; eauto); contradiction.
-Qed.
+    Definition NP3T := NaivePair3 (E_Trace zero E_Nat) (E_Trace one E_Nat) (E_Trace two E_Nat).
+    Eval compute in Trace_lt NP3T 14.
+    Eval compute in sqrt (sqrt 7).
 
-Definition traceNP3 := Trace_lt (NaivePair3 (E_Trace zero E_Nat) (E_Trace one E_Nat) (E_Trace two E_Nat)).
+    Theorem NaivePairUnFair : ~ (Fair3 NaivePair3).
+    Proof.
 
-Lemma z_to_n_nosubS m : ~ subset (z_to_n (S m)) (z_to_n m).
-Proof.
-  intros H.
-  assert (set_In m (z_to_n m)).
-  eapply In_subset_def; eauto.
-  apply z_to_n_correct; nliamega.
-  rewrite z_to_n_correct in H0.
-  nliamega.
-Qed.
+      apply AltUnfair3Suff.
+      unfold AltUnfair3.
+      fold NP3T.
+      exists 15.
+      intros n H.
+      assert (16 <= n) as H' by nliamega ; clear H.
+      remember (Trace_lt NP3T n) as t; destruct t as [t0 t1 t2 t3].
+      destruct (sqrt_spec_2 n) as [m [p [[Hmn Hnp] Hppmm]]]; auto.
 
-Lemma z_to_n_nosub' m n : ~ subset (z_to_n (S (m + n))) (z_to_n m).
-Proof.
-  induction n.
-  replace (m + 0) with m by nliamega.
-  apply z_to_n_nosubS.
-  unfold z_to_n; fold z_to_n.
-  replace (m + S n) with (S (m + n)) by nliamega.
-  intros H.
-  apply IHn.
-  apply subset_In_def.
-  intros x.
-  rewrite z_to_n_correct.
-  intros Hlt.
-  assert (set_In x (set_add' (S (m + n)) (z_to_n (S (m + n))))).
-  replace (set_add' (S (m + n)) (z_to_n (S (m + n)))) with (z_to_n (S (S (m + n)))).
-  apply z_to_n_correct; nliamega.
-  trivial.
-  eapply In_subset_def.
-  apply H.
-  auto.
-Qed.
+      left.
+      assert (~ subset t0 t1); [ | intros []; contradiction].
 
-Lemma z_to_n_nosub m n : m < n -> ~ subset (z_to_n n) (z_to_n m).
-Proof.
-  intros H1 H2.
-  destruct n; [nliamega|].
-  assert (n < m); [| nliamega].
-  apply z_to_n_correct.
-  eapply In_subset_def.
-  eapply subset_trans; eauto.
-  unfold set_In.
-  rewrite !z_to_n_correct; auto.
-Qed.
+      assert (subset (z_to_n m) t0).
+      - remember (Trace_lt NP3T (m * m)) as t; destruct t as [mm0 mm1 mm2 mm3].
+        assert (sub_trace (Trace_lt NP3T (m * m)) (Trace_lt NP3T n))
+          by (apply Trace_lt_sub; auto).
+        unfold sub_trace in H.
+        rewrite <-Heqt in H.
+        rewrite <-Heqt0 in H.
+        destruct4 H.
+        eapply subset_trans; try eassumption.
+        clear H H0 H1 H2; clear dependent t0; clear t1 t2 t3.
+        unfold NP3T, NaivePair3 in *.
+        remember (Pair_precise m (E_Trace zero E_Nat) (E_Pair (E_Trace one E_Nat) (E_Trace two E_Nat))).
+        clear Heqt.
+        rewrite <-Heqt0 in t.
+        remember ((trace_plus (Trace_lt (E_Trace zero E_Nat) m) (Trace_lt (E_Pair (E_Trace one E_Nat) (E_Trace two E_Nat)) m))).
+        destruct t0.
+        replace mm0 with (trace_proj zero (Tracing mm0 mm1 mm2 mm3)) by auto.
+        eapply subset_trans; [| apply trace_eq_proj;  eassumption].
+        rewrite Heqt1.
+        rewrite trace_proj_plus_distrl.
+        apply subset_union_transl.
+        apply trace_lt_Nat.
 
-Definition NP3T := NaivePair3 (E_Trace zero E_Nat) (E_Trace one E_Nat) (E_Trace two E_Nat).
-Eval compute in Trace_lt NP3T 14.
-Eval compute in sqrt (sqrt 7).
-
-Lemma sqrt_slower_than_id' n :
-  (S (sqrt (S (4 + n)))) < 4 + n.
-Proof.
-  induction n.
-  compute; reflexivity.
-  assert (sqrt (S (4 + S n)) <= (S (S (S n)))); [| nliamega].
-  eapply le_trans; [apply Nat.sqrt_succ_le|].
-  replace (4 + S n) with (S (4 + n)) by nliamega.
-  nliamega.
-Qed.
-
-Lemma sqrt_slower_than_id n :
-  4 <= n ->
-  (S (sqrt (S n))) < n.
-Proof.
-  intros H.
-  replace n with (4 + (n - 4)) by nliamega.
-  apply sqrt_slower_than_id'.
-Qed.
-
-Lemma sqrt_spec_2 n :
-  16 <= n ->
-  exists m p,
-    m * m <= n < (p * p) * (p * p) /\ p * p < m * m.
-Proof.
-  intros H.
-  exists (S (S (sqrt (S (sqrt n))))).
-  exists (S (sqrt (S (sqrt n)))).
-  split; [| nliamega].
-  split; [| destruct (sqrt_spec n); destruct (sqrt_spec (S (sqrt n))); nliamega ].
-  destruct (sqrt_spec n).
-  apply le_trans with (m := sqrt n * sqrt n); auto.
-  assert (S (S (sqrt (S (sqrt n)))) <= sqrt n) as Hperf; [|(apply mult_le_compat; apply Hperf)].
-  assert (4 <= sqrt n).
-  replace 4 with (sqrt 16) .
-  apply Nat.sqrt_le_mono; auto.
-  compute; trivial.
-  apply sqrt_slower_than_id; auto.
-Qed.
-
-Lemma nat_le_iff : forall m p, (forall q : nat, q <= m -> q <= p) <-> m <= p.
-Proof.
-  split.
-  intros H. apply (H m); auto.
-  intros H q; nliamega.
-Qed.
-
-Lemma nat_lt_iff : forall m p, (forall q : nat, q < m -> q < p) <-> m <= p.
-Proof.
-  destruct m.
-  intros p; split; [nliamega| intros _ q contra; inversion contra].
-  destruct p.
-  split.
-  intros contra; assert (m < 0) by (apply contra; auto); nliamega.
-  intros contra; inversion contra.
-  split.
-  intros H.
-  assert (m <= p); [| nliamega].
-  apply nat_le_iff.
-  intros q Hqm.
-  assert (q < S p); [| nliamega].
-  apply H; nliamega.
-  intros; nliamega.
-Qed.
-
-Theorem PairPairUnFair : ~ (Fair3 NaivePair3).
-Proof.
-
-  apply AltUnfair3Suff.
-  unfold AltUnfair3.
-  fold NP3T.
-  exists 15.
-  intros n H.
-  assert (16 <= n) as H' by nliamega ; clear H.
-  remember (Trace_lt NP3T n) as t; destruct t as [t0 t1 t2 t3].
-  destruct (sqrt_spec_2 n) as [m [p [[Hmn Hnp] Hppmm]]]; auto.
-
-  left.
-  assert (~ subset t0 t1); [ | intros []; contradiction].
-
-  assert (subset (z_to_n m) t0).
-  - remember (Trace_lt NP3T (m * m)) as t; destruct t as [mm0 mm1 mm2 mm3].
-    assert (sub_trace (Trace_lt NP3T (m * m)) (Trace_lt NP3T n))
-      by (apply Trace_lt_sub; auto).
-    unfold sub_trace in H.
-    rewrite <-Heqt in H.
-    rewrite <-Heqt0 in H.
-    destruct4 H.
-    eapply subset_trans; try eassumption.
-    clear H H0 H1 H2; clear dependent t0; clear t1 t2 t3.
-    unfold NP3T, NaivePair3 in *.
-    remember (Pair_precise m (E_Trace zero E_Nat) (E_Pair (E_Trace one E_Nat) (E_Trace two E_Nat))).
-    clear Heqt.
-    rewrite <-Heqt0 in t.
-    remember ((trace_plus (Trace_lt (E_Trace zero E_Nat) m) (Trace_lt (E_Pair (E_Trace one E_Nat) (E_Trace two E_Nat)) m))).
-    destruct t0.
-    replace mm0 with (trace_proj zero (Tracing mm0 mm1 mm2 mm3)) by auto.
-    eapply subset_trans; [| apply trace_eq_proj;  eassumption].
-    rewrite Heqt1.
-    rewrite trace_proj_plus_distrl.
-    apply subset_union_transl.
-    apply trace_lt_Nat.
-
-  - assert (subset t1 (z_to_n p)).
-    remember (Trace_lt NP3T ((p * p) * (p * p))) as p4t.
-    assert (sub_trace (Trace_lt NP3T n) p4t) by (subst; apply Trace_lt_sub; auto; nliamega).
-    destruct p4t as [pt0 pt1 pt2 pt3].
-    unfold sub_trace in H0.
-    rewrite <-Heqt in H0.
-    destruct4 H0.
-    eapply subset_trans; try eassumption.
-    clear H0 H1 H2 H3; clear dependent t0; clear t1 t2 t3; clear dependent m; clear dependent n.
-    unfold NP3T in Heqp4t.
-    unfold NaivePair3 in Heqp4t.
-    remember (PairPair_precise p (E_Trace zero E_Nat) (E_Trace one E_Nat) (E_Trace two E_Nat)).
-    clear Heqt.
-    rewrite <-Heqp4t in t.
-    apply set_subset_weaken.
-    replace pt1 with (trace_proj one (Tracing pt0 pt1 pt2 pt3)) by trivial.
-    clear Heqp4t.
-    eapply set_eq_trans.
-    apply trace_eq_proj.
-    apply t.
-    apply set_eq_symm.
-    eapply set_eq_trans.
-    apply trace_lt_Nat with (tg := one).
-    rewrite trace_proj_plus_distrl.
-    rewrite trace_proj_plus_distrl.
-    rewrite trace_lt_Nat_off with (tg2 := zero); [| discriminate].
-    rewrite trace_lt_Nat_off with (tg2 := two); [| discriminate].
-    apply set_eq_symm.
-    eapply set_eq_trans; [apply set_union_unitl|].
-    eapply set_eq_trans; [apply set_union_unitr|].
-    apply set_eq_refl.
-    intros Hsub01.
-    assert (subset (z_to_n m) (z_to_n p)).
-    eapply subset_trans; try eassumption.
-    eapply subset_trans; try eassumption.
-    assert (m <= p); [| nliamega].
-    apply nat_lt_iff.
-    intros q.
-    rewrite <-z_to_n_correct.
-    rewrite <-z_to_n_correct.
-    apply In_subset_def; assumption.
-Qed.
-
+      - assert (subset t1 (z_to_n p)).
+        remember (Trace_lt NP3T ((p * p) * (p * p))) as p4t.
+        assert (sub_trace (Trace_lt NP3T n) p4t) by (subst; apply Trace_lt_sub; auto; nliamega).
+        destruct p4t as [pt0 pt1 pt2 pt3].
+        unfold sub_trace in H0.
+        rewrite <-Heqt in H0.
+        destruct4 H0.
+        eapply subset_trans; try eassumption.
+        clear H0 H1 H2 H3; clear dependent t0; clear t1 t2 t3; clear dependent m; clear dependent n.
+        unfold NP3T in Heqp4t.
+        unfold NaivePair3 in Heqp4t.
+        remember (PairPair_precise p (E_Trace zero E_Nat) (E_Trace one E_Nat) (E_Trace two E_Nat)).
+        clear Heqt.
+        rewrite <-Heqp4t in t.
+        apply set_subset_weaken.
+        replace pt1 with (trace_proj one (Tracing pt0 pt1 pt2 pt3)) by trivial.
+        clear Heqp4t.
+        eapply set_eq_trans.
+        apply trace_eq_proj.
+        apply t.
+        apply set_eq_symm.
+        eapply set_eq_trans.
+        apply trace_lt_Nat with (tg := one).
+        rewrite trace_proj_plus_distrl.
+        rewrite trace_proj_plus_distrl.
+        rewrite trace_lt_Nat_off with (tg2 := zero); [| discriminate].
+        rewrite trace_lt_Nat_off with (tg2 := two); [| discriminate].
+        apply set_eq_symm.
+        eapply set_eq_trans; [apply set_union_unitl|].
+        eapply set_eq_trans; [apply set_union_unitr|].
+        apply set_eq_refl.
+        intros Hsub01.
+        assert (subset (z_to_n m) (z_to_n p)).
+        eapply subset_trans; try eassumption.
+        eapply subset_trans; try eassumption.
+        assert (m <= p); [| nliamega].
+        apply nat_lt_iff.
+        intros q.
+        rewrite <-z_to_n_correct.
+        rewrite <-z_to_n_correct.
+        apply In_subset_def; assumption.
+    Qed.
+  End NaivePairUnfair.
+End Fairness.
 Recursive Extraction Enumerates_to_dec Enumerates_from_dec.
